WP1-Programming-Languages-Semantics/WP11-C-semantics/src/IMP-Lenses/Algebraic_Laws.thy
@@ -6,7 +6,7 @@ text{*In this section we introduce the semantic rules related to the different
       language, and this before any deductive proof verification activity or formal testing.*}
 
 theory Algebraic_Laws
-imports Commands
+imports Commands "utp/utp_urel_laws"
 begin
 
 named_theorems small_step(*legacy*) and  symbolic_exec_subst
@@ -16,956 +16,618 @@ subsection {*SKIP Laws*}
 text{*In this section we introduce the algebraic laws of programming related to the SKIP
       statement.*}
 
-lemma SKI0 [symbolic_exec_subst]:
-  "SKIP ; C = C"
-  by auto
+lemma seqr_left_unit [simp, symbolic_exec_subst]:
+  "SKIP ;; P = P"
+  unfolding skip_r_def
+  by transfer auto
 
-lemma SKI1[symbolic_exec_subst]:
-  "C ; SKIP = C"
-  by auto
+lemma seqr_right_unit [simp, symbolic_exec_subst]:
+  "P ;; SKIP = P"
+  unfolding skip_r_def
+  by transfer auto
+
+lemma pre_skip_post: "(\<lceil>b\<rceil>\<^sub>< \<and> SKIP) = (SKIP \<and> \<lceil>b\<rceil>\<^sub>>)"
+  unfolding skip_r_def
+  by (rel_auto)
+
+lemma skip_var:
+  fixes x :: "(bool, '\<alpha>) uvar"
+  shows "($x \<and> SKIP) = (SKIP \<and> $x\<acute>)"
+   unfolding skip_r_def
+  by (rel_auto)
+
+lemma assign_r_alt_def:
+  fixes x :: "('a, '\<alpha>) uvar"
+  shows "x :== v = SKIP\<lbrakk>\<lceil>v\<rceil>\<^sub></$x\<rbrakk> "
+  unfolding cond_def skip_r_def
+  by rel_auto
+
+lemma skip_r_alpha_eq:
+  "SKIP = ($\<Sigma>\<acute> =\<^sub>u $\<Sigma>)"
+  unfolding  skip_r_def
+  by (rel_auto)
 
 subsection {*Assignment Laws*}
 text{*In this section we introduce the algebraic laws of programming related to the assignment
       statement.*}
 
-lemma ASN_test:
+lemma "&v\<lbrakk>expr/v\<rbrakk> = [v \<mapsto>\<^sub>s expr] \<dagger> &v" ..
+
+lemma usubst_cancel[usubst,symbolic_exec_subst]: 
+  assumes 1:"weak_lens v" 
+  shows "(&v)\<lbrakk>expr/v\<rbrakk>= expr"
+  using 1
+  by transfer' rel_auto
+
+lemma usubst_cancel_r[usubst,symbolic_exec_subst]: 
+  assumes 1:"weak_lens v" 
+  shows "($v)\<lbrakk>\<lceil>expr\<rceil>\<^sub></$v\<rbrakk>= \<lceil>expr\<rceil>\<^sub><"
+  using 1
+  by transfer' rel_auto
+
+lemma assign_test:
   assumes 1:"mwb_lens x" 
-  shows     "(x :== \<guillemotleft>u\<guillemotright> ; x :== \<guillemotleft>v\<guillemotright>) = (x :== \<guillemotleft>v\<guillemotright>)"
-  using 1 unfolding subst_upd_var_def 
-  by transfer auto
+  shows     "(x :== \<guillemotleft>u\<guillemotright> ;; x :== \<guillemotleft>v\<guillemotright>) = (x :== \<guillemotleft>v\<guillemotright>)"
+  using 1   
+  by (simp add: assigns_comp subst_upd_comp subst_lit usubst_upd_idem)
 
-lemma ASN_cancel:
-  assumes 1:"weak_lens var" 
-  shows "(var :== expr)\<dagger> (VAR var) = expr"
-  using 1 unfolding subst_upd_var_def
-  by transfer auto
+lemma assign_r_comp[symbolic_exec_subst]: 
+  "(x :== u ;; P) = P\<lbrakk>\<lceil>u\<rceil>\<^sub></$x\<rbrakk>" (*legacy: mwb_lens x \<Longrightarrow>*)
+  by (simp add: assigns_r_comp usubst)
 
-lemma ASN0[small_step]:
-  "(var:== exp ; C) = C o [var \<mapsto>\<^sub>s exp]" ..
+lemma assign_twice[symbolic_exec_subst]: 
+  assumes "mwb_lens x" and  "x \<sharp> f" (*legacy: vwb_lens x *)
+  shows "(x :== e ;; x :== f) = (x :== f)" 
+  using assms
+  by (simp add: assigns_comp usubst)
 
-lemma ASN1[small_step]: 
-  "(var:== exp ; C) \<dagger> P = [var \<mapsto>\<^sub>s exp] \<dagger> (C \<dagger> P)"
-  by transfer simp
- 
-lemma ASN2[small_step]: 
-  "(var:== exp ; C) = [var \<mapsto>\<^sub>s exp] \<dagger> C"
-  unfolding SKI1 subst_subst
-  by transfer auto 
+lemma assign_commute:
+  assumes "x \<bowtie> y" "x \<sharp> f" "y \<sharp> e"
+  shows "(x :== e ;; y :== f) = (y :== f ;; x :== e)"
+  using assms
+  by (rel_auto, simp_all add: lens_indep_comm)
 
-lemma ASN3[small_step]: 
-  assumes 1:"var \<sharp>\<sharp> C"
-  shows"(var:== exp ; C) = C (var \<mapsto>\<^sub>s exp)"
-  using 1 unfolding unrest_usubst_def ASN2 SKI1 subst_upd_var_def 
-  by transfer auto 
+lemma assign_cond:
+  fixes x :: "('a, '\<alpha>) uvar"
+  assumes "out\<alpha> \<sharp> b"
+  shows "(x :== e ;; (IF b THEN P ELSE Q)) = 
+         (IF (b\<lbrakk>\<lceil>e\<rceil>\<^sub></$x\<rbrakk>) THEN (x :== e ;; P) ELSE (x :== e ;; Q))"
+  unfolding cond_def
+  by rel_auto
 
-text {*In the sequel we find assign laws which are in Simon Foster paper*}
-text {*The rules in the sequel are too generic. 
-       We can not use these rules naively in an automatic tactic for optimizing the program. 
-       To be applied to a given program this rule needs some knowledge, eg., annotations
-       saying that @{text "var \<sharp> exp2"} is true.*}
+lemma assign_rcond:
+  fixes x :: "('a, '\<alpha>) uvar"
+  shows "(x :== e ;; (P \<triangleleft> b \<triangleright>\<^sub>r Q)) = ((x :== e ;; P) \<triangleleft> (b\<lbrakk>e/x\<rbrakk>) \<triangleright>\<^sub>r (x :== e ;; Q))"
+  unfolding cond_def
+  by rel_auto
 
-lemma ASN4: 
-  assumes 1: "mwb_lens var" 
-  and  2: "var \<sharp> exp2" (*Thats why he needs the concept of unrest in his theory*)
-  shows "(var:== exp1 ; var:== exp2) = var:== exp2" 
-proof (rule ext)
-  fix \<sigma> :: 'b
-  have "\<forall>u \<sigma> v. put\<^bsub>var\<^esub> \<sigma> v = put\<^bsub>var\<^esub> (put\<^bsub>var\<^esub> \<sigma> u) v"
-    using 1 by auto
-  then have "subst_upd SKIP var exp2 \<sigma> = 
-             subst_upd SKIP var exp2 (subst_upd SKIP var exp1 \<sigma>)"
-    using 2
-    by (auto simp add: subst_upd_var_def  unrest.abs_eq)
-  then show "(subst_upd SKIP var exp1; subst_upd SKIP var exp2) \<sigma> = 
-              subst_upd SKIP var exp2 \<sigma>"
-    by (simp add: subst.abs_eq) 
-qed
+term "v:== uop F (&v)"
+term "uop F ($v)"
+term"(v:== e1 ;; v:== (uop F (&v))) = (v:== (uop F e1))"
+lemma assign_uop1[symbolic_exec_subst]: 
+  assumes 1: "mwb_lens v"
+  shows "(v:== e1 ;; v:== (uop F (&v))) = (v:== (uop F e1))"
+  using 1 
+  by rel_auto
 
-lemma ASN4_uop1[symbolic_exec_subst]: 
-  assumes 1: "mwb_lens var"
-  shows "(var:== exp1 ; var:== (uop F (VAR var))) = (var:== (uop F exp1))"
-  using 1  unfolding subst_upd_var_def unrest_def
-  by transfer auto 
+lemma assign_bop1: 
+  assumes 1: "mwb_lens v" and 2:"v \<sharp> e2"
+  shows "(v:== e1 ;; v:== (bop bp (&v) e2)) = (v:== (bop bp e1 e2))"
+  using 1 2  
+  by rel_auto
 
-lemma ASN4_bop1: 
-  assumes 1: "mwb_lens var" and 2:"var \<sharp> exp2"
-  shows "(var:== exp1 ; var:== (bop bp (VAR var) exp2)) = (var:== (bop bp exp1 exp2))"
-  using 1 2  unfolding subst_upd_var_def unrest_def
-  by transfer auto
+lemma assign_bop2: 
+  assumes 1: "mwb_lens v" and 2:"v \<sharp> e2"
+  shows "(v:== e1 ;; v:== (bop bp e2 (&v))) = (v:== (bop bp e2 e1))"
+  using 1 2  
+  by rel_auto
 
-lemma ASN4_bop2: 
-  assumes 1: "mwb_lens var" and 2:"var \<sharp> exp2"
-  shows "(var:== exp1 ; var:== (bop bp exp2 (VAR var))) = (var:== (bop bp exp2 exp1))"
-  using 1 2 unfolding subst_upd_var_def unrest_def
-  by transfer auto
+lemma assign_trop1: 
+  assumes 1: "mwb_lens v" and 2:"v \<sharp> e2" and 3:"v \<sharp> e3"
+  shows "(v:== e1 ;; v:== (trop tp (&v) e2 e3)) = 
+         (v:== (trop tp e1 e2 e3))"
+  using 1 2 3
+  by rel_auto
 
-lemma ASN4_trop1: 
-  assumes 1: "mwb_lens var" and 2:"var \<sharp> exp2" and 3:"var \<sharp> exp3"
-  shows "(var:== exp1 ; var:== (trop tp (VAR var) exp2 exp3)) = 
-         (var:== (trop tp exp1 exp2 exp3))"
-  using 1 2 3 unfolding subst_upd_var_def unrest_def
-  by transfer auto
+lemma assign_trop2: 
+  assumes 1: "mwb_lens v" and 2:"v \<sharp> e2" and 3:"v \<sharp> e3"
+  shows "(v:== e1 ;; v:== (trop tp e2 (&v) e3)) = 
+         (v:== (trop tp e2 e1 e3))"
+  using 1 2 3
+  by rel_auto
 
-lemma ASN4_trop2: 
-  assumes 1: "mwb_lens var" and 2:"var \<sharp> exp2" and 3:"var \<sharp> exp3"
-  shows "(var:== exp1 ; var:== (trop tp exp2 (VAR var) exp3)) = 
-         (var:== (trop tp exp2 exp1 exp3))"
-  using 1 2 3 unfolding subst_upd_var_def unrest_def
-  by transfer auto
+lemma assign_trop3: 
+  assumes 1: "mwb_lens v" and 2:"v \<sharp> e2" and 3:"v \<sharp> e3"
+  shows "(v:== e1 ;; v:== (trop tp e2 e3 (&v))) = 
+         (v:== (trop tp e2 e3 e1))"
+  using 1 2 3
+  by rel_auto
 
-lemma ASN4_trop3: 
-  assumes 1: "mwb_lens var" and 2:"var \<sharp> exp2" and 3:"var \<sharp> exp3"
-  shows "(var:== exp1 ; var:== (trop tp exp2 exp3 (VAR var))) = 
-         (var:== (trop tp exp2 exp3 exp1))"
-  using 1 2 3 unfolding subst_upd_var_def unrest_def
-  by transfer auto
+lemma assign_qtop1: 
+  assumes 1: "mwb_lens v" and 2:"v \<sharp> e2" and 3:"v \<sharp> e3" and 4:"v \<sharp> e4"
+  shows "(v:== e1 ;; v:== (qtop tp (&v) e2 e3 e4)) = 
+         (v:== (qtop tp e1 e2 e3 e4))"
+  using 1 2 3 4
+  by rel_auto
 
-lemma ASN4_qtop1: 
-  assumes 1: "mwb_lens var" and 2:"var \<sharp> exp2" and 3:"var \<sharp> exp3" and 4:"var \<sharp> exp4"
-  shows "(var:== exp1 ; var:== (qtop tp (VAR var) exp2 exp3 exp4)) = 
-         (var:== (qtop tp exp1 exp2 exp3 exp4))"
-  using 1 2 3 4 unfolding subst_upd_var_def unrest_def
-  by transfer auto
+lemma assign_qtop2: 
+  assumes 1: "mwb_lens v" and 2:"v \<sharp> e2" and 3:"v \<sharp> e3" and 4:"v \<sharp> e4"
+  shows "(v:== e1 ;; v:== (qtop tp e2 (&v) e3 e4)) = 
+         (v:== (qtop tp e2 e1 e3 e4))"
+  using 1 2 3 4
+  by rel_auto
 
-lemma ASN4_qtop2: 
-  assumes 1: "mwb_lens var" and 2:"var \<sharp> exp2" and 3:"var \<sharp> exp3" and 4:"var \<sharp> exp4"
-  shows "(var:== exp1 ; var:== (qtop tp exp2 (VAR var) exp3 exp4)) = 
-         (var:== (qtop tp exp2 exp1 exp3 exp4))"
-  using 1 2 3 4 unfolding subst_upd_var_def unrest_def
-  by transfer auto
+lemma assign_qtop3: 
+  assumes 1: "mwb_lens v" and 2:"v \<sharp> e2" and 3:"v \<sharp> e3" and 4:"v \<sharp> e4"
+  shows "(v:== e1 ;; v:== (qtop tp e2 e3 (&v) e4)) = 
+         (v:== (qtop tp e2 e3 e1 e4))"
+  using 1 2 3 4
+  by rel_auto
 
-lemma ASN4_qtop3: 
-  assumes 1: "mwb_lens var" and 2:"var \<sharp> exp2" and 3:"var \<sharp> exp3" and 4:"var \<sharp> exp4"
-  shows "(var:== exp1 ; var:== (qtop tp exp2 exp3 (VAR var) exp4)) = 
-         (var:== (qtop tp exp2 exp3 exp1 exp4))"
-  using 1 2 3 4 unfolding subst_upd_var_def unrest_def
-  by transfer auto
+lemma assign_qtop4: 
+  assumes 1: "mwb_lens v" and 2:"v \<sharp> e2" and 3:"v \<sharp> e3" and 4:"v \<sharp> e4"
+  shows "(v:== e1 ;; v:== (qtop tp e2 e3 e4 (&v))) = 
+         (v:== (qtop tp e2 e3 e4 e1))"
+  using 1 2 3 4
+  by rel_auto
 
-lemma ASN4_qtop4: 
-  assumes 1: "mwb_lens var" and 2:"var \<sharp> exp2" and 3:"var \<sharp> exp3" and 4:"var \<sharp> exp4"
-  shows "(var:== exp1 ; var:== (qtop tp exp2 exp3 exp4 (VAR var))) = 
-         (var:== (qtop tp exp2 exp3 exp4 exp1))"
-  using 1 2 3 4 unfolding subst_upd_var_def unrest_def
-  by transfer auto
-
-lemma ASN5:
-  assumes  1: "var1 \<sharp> exp2"
-  and  2: "var2 \<sharp> exp1"
-  and  3: "var1 \<bowtie> var2"
-  shows "(var1:== exp1 ; var2:== exp2) = (var2:== exp2 ; var1:== exp1)" 
-proof (rule ext)
-  fix \<sigma> :: 'b
-  have h1: "\<And>subst var \<sigma> v. subst_upd subst (var::'a \<Longrightarrow> 'b) exp1 (put\<^bsub>var2\<^esub> \<sigma> v) = 
-           put\<^bsub>var\<^esub> (subst (put\<^bsub>var2\<^esub> \<sigma> v)) (exp1 \<sigma>)"
-    using 2 by (simp add: unrest.abs_eq subst_upd_var_def) 
-  have "var1 \<bowtie> var2" 
-    using 3 by simp
-  then have "put\<^bsub>var1\<^esub> (put\<^bsub>var2\<^esub> \<sigma> (exp2 \<sigma>)) (exp1 \<sigma>) = 
-             put\<^bsub>var2\<^esub> (put\<^bsub>var1\<^esub> \<sigma> (exp1 \<sigma>)) (exp2 \<sigma>)"
-    by (simp add: lens_indep_comm)
-  then have "subst_upd SKIP var2 exp2 (put\<^bsub>var1\<^esub> \<sigma> (exp1 \<sigma>)) = 
-             put\<^bsub>var1\<^esub> (put\<^bsub>var2\<^esub> \<sigma> (exp2 \<sigma>)) (exp1 \<sigma>)"
-    using 1 unfolding subst_upd_var_def by transfer simp
-  then have "(subst_upd SKIP var1 exp1; subst_upd SKIP var2 exp2) \<sigma> = 
-             put\<^bsub>var1\<^esub> (put\<^bsub>var2\<^esub> \<sigma> (exp2 \<sigma>)) (exp1 \<sigma>)"
-    unfolding subst_upd_var_def by transfer simp
-  then have "(subst_upd SKIP var1 exp1; subst_upd SKIP var2 exp2) \<sigma> = 
-              subst_upd SKIP var1 exp1 (put\<^bsub>var2\<^esub> \<sigma> (exp2 \<sigma>))"
-    using h1 by simp
-  then show "(subst_upd SKIP var1 exp1; subst_upd SKIP var2 exp2) \<sigma> = 
-             (subst_upd SKIP var2 exp2; subst_upd SKIP var1 exp1) \<sigma>"
-    unfolding subst_upd_var_def by transfer simp
-qed
-
-lemma ASN6[symbolic_exec_subst]:
-  "(IF ([var \<mapsto>\<^sub>s exp] \<dagger> bexp) THEN (var:== exp ; C1) ELSE (var:== exp ; C2)) = 
-   (var:== exp ; IF bexp THEN C1 ELSE C2)" 
-  by transfer auto
+lemma assign_cond_seqr_dist[symbolic_exec_subst]:
+  "(IF (b\<lbrakk>\<lceil>e\<rceil>\<^sub></$v\<rbrakk>) THEN (v:== e ;; P) ELSE (v:== e ;; Q)) = 
+   (v:== e ;; IF b THEN P ELSE Q)" 
+  unfolding cond_def
+  by rel_auto
 
 text {*In the sequel we find assignment laws proposed by Hoare*}
 
-lemma ASN8:
-  assumes 1: "vwb_lens var"
-  shows "(var:== VAR var) = SKIP"
-  using 1 usubst_upd_var_id [of var]
-  by simp
+lemma assign_vwb_skip:
+  assumes 1: "vwb_lens v"
+  shows "(v:== &v) = SKIP"
+  by (simp add: assms skip_r_def usubst_upd_var_id)
 
-lemma ASN9:
-  assumes 1: "mwb_lens var1"
-  and     2: "vwb_lens var2"
-  and     3: "var1 \<bowtie> var2"
-  shows"[var1 \<mapsto>\<^sub>s exp, var2 \<mapsto>\<^sub>s (VAR var2)] = (var1:== exp)"
-  using 1 2 3 unfolding subst_upd_var_def subst.abs_eq imp_var.abs_eq id_def
-proof -
-  { fix \<sigma> :: 'b
-    have "put\<^bsub>var1\<^esub> \<sigma> (exp \<sigma>) = put\<^bsub>var2\<^esub> (put\<^bsub>var1\<^esub> \<sigma> (exp \<sigma>)) (get\<^bsub>var2\<^esub> \<sigma>)"
-      using 3 2 lens_indep_comm
-      by (metis vwb_lens_wb wb_lens.get_put)
- }
-  then show "(\<lambda>\<sigma>. put\<^bsub>var2\<^esub> (put\<^bsub>var1\<^esub> \<sigma> (exp \<sigma>)) (get\<^bsub>var2\<^esub> \<sigma>)) = 
-             (\<lambda>\<sigma>. put\<^bsub>var1\<^esub> \<sigma> (exp \<sigma>))" 
-    by auto
-qed
-
-lemma ASN10[small_step]:
+lemma assign_simultanious:
   assumes  1: "vwb_lens var2"
-  shows"(var1:== exp); (var2 :== (VAR var2)) = (var1:== exp)"
-  using 1 ASN8[of var2]
-  by simp 
+  and     2: "var1 \<bowtie> var2"
+  shows"(var1, var2 :== exp , &var2) = (var1 :== exp)"
+  by (simp add: "1" "2" usubst_upd_comm usubst_upd_var_id)
 
-lemma ASN11_uop[symbolic_exec_subst]:
-  assumes 1: "weak_lens var"
-  shows "(IF (uop F exp) THEN (var:== exp ; C1) ELSE (var:== exp ; C2)) = 
-         (var:== exp ; IF (uop F (VAR var)) THEN C1 ELSE C2)"
-  using 1 unfolding subst_upd_var_def 
-  by transfer auto 
+lemma assign_seq[small_step]:
+  assumes  1: "vwb_lens var2"
+  shows"(var1:== exp);; (var2 :== &var2) = (var1:== exp)"
+  using 1 by rel_auto
 
-lemma ASN11_bop1:
-  assumes 1: "weak_lens var" and 2: "var \<sharp> exp2"
-  shows "(var:== exp ; IF (bop bp (VAR var) exp2) THEN C1 ELSE C2) = 
-         (IF (bop bp exp exp2) THEN (var:== exp ; C1) ELSE (var:== exp ; C2))"
-  using 1 2 unfolding subst_upd_var_def unrest_def
-  by transfer auto
+lemma assign_cond_uop[symbolic_exec_subst]:
+  assumes 1: "weak_lens v"
+  shows "(v:== exp ;; C1) \<triangleleft>uop F exp\<triangleright>\<^sub>r (v:== exp ;; C2) = 
+          v:== exp ;; C1 \<triangleleft>uop F (&v)\<triangleright>\<^sub>r  C2"
+  using 1 unfolding cond_def
+  by rel_auto
 
-lemma ASN11_bop2:
-  assumes 1: "weak_lens var" and 2: "var \<sharp> exp2"
-  shows "(var:== exp1 ; IF (bop bp exp2 (VAR var)) THEN C1 ELSE C2) = 
-         (IF (bop bp exp2 exp1) THEN (var:== exp1 ; C1) ELSE (var:== exp1 ; C2))"
-  using 1 2 unfolding subst_upd_var_def unrest_def
-  by transfer auto
+lemma assign_cond_bop1:
+  assumes 1: "weak_lens v" and 2: "v \<sharp> exp2"
+  shows "(v:== exp ;; C1 \<triangleleft>(bop bp (&v) exp2)\<triangleright>\<^sub>r C2) = 
+         ((v:== exp ;; C1) \<triangleleft>(bop bp exp exp2)\<triangleright>\<^sub>r  (v:== exp ;; C2))"
+  using 1 2 unfolding cond_def
+  by rel_auto
 
-lemma ASN11_trop1:
-  assumes 1: "weak_lens var" and 2: "var \<sharp> exp2" and 3: "var \<sharp> exp3"
-  shows "(var:== exp ; IF (trop tp (VAR var) exp2 exp3) THEN C1 ELSE C2) = 
-         (IF (trop tp exp exp2 exp3) THEN (var:== exp ; C1) ELSE (var:== exp ; C2))"
-  using 1 2 3 unfolding subst_upd_var_def unrest_def
-  by transfer auto
+lemma assign_cond_bop2:
+  assumes 1: "weak_lens v" and 2: "v \<sharp> exp2"
+  shows "(v:== exp1 ;; C1 \<triangleleft>(bop bp exp2 (&v))\<triangleright>\<^sub>r C2) = 
+         ((v:== exp1 ;; C1) \<triangleleft>(bop bp exp2 exp1)\<triangleright>\<^sub>r (v:== exp1 ;; C2))"
+  using 1 2 unfolding cond_def
+  by rel_auto
 
-lemma ASN11_trop2:
-  assumes 1: "weak_lens var" and 2: "var \<sharp> exp2" and 3: "var \<sharp> exp3"
-  shows "(var:== exp1 ; IF (trop tp exp2 (VAR var) exp3) THEN C1 ELSE C2) = 
-         (IF (trop tp exp2 exp1 exp3) THEN (var:== exp1 ; C1) ELSE (var:== exp1 ; C2))"
-  using 1 2 3 unfolding subst_upd_var_def unrest_def
-  by transfer auto
+lemma assign_cond_trop1:
+  assumes 1: "weak_lens v" and 2: "v \<sharp> exp2" and 3: "v \<sharp> exp3"
+  shows "(v:== exp ;; C1 \<triangleleft>(trop tp (&v) exp2 exp3)\<triangleright>\<^sub>r C2) = 
+         ((v:== exp ;; C1) \<triangleleft>(trop tp exp exp2 exp3)\<triangleright>\<^sub>r (v:== exp ;; C2))"
+  using 1 2 3 unfolding cond_def
+  by rel_auto
 
-lemma ASN11_trop3:
-  assumes 1: "weak_lens var" and 2: "var \<sharp> exp2" and 3: "var \<sharp> exp3"
-  shows "(var:== exp1 ; IF (trop bp exp2 exp3 (VAR var)) THEN C1 ELSE C2) = 
-         (IF (trop bp exp2 exp3 exp1) THEN (var:== exp1 ; C1) ELSE (var:== exp1 ; C2))"
-  using 1 2 3 unfolding subst_upd_var_def unrest_def
-  by transfer auto
+lemma assign_cond_trop2:
+  assumes 1: "weak_lens v" and 2: "v \<sharp> exp2" and 3: "v \<sharp> exp3"
+  shows "(v:== exp1 ;; C1 \<triangleleft>(trop tp exp2 (&v) exp3)\<triangleright>\<^sub>r C2) = 
+         ((v:== exp1 ;; C1) \<triangleleft>(trop tp exp2 exp1 exp3)\<triangleright>\<^sub>r (v:== exp1 ;; C2))"
+  using 1 2 3 unfolding cond_def
+  by rel_auto
 
-lemma ASN11_qtop1:
-  assumes 1: "weak_lens var" and 2: "var \<sharp> exp2" and 3: "var \<sharp> exp3" and 4: "var \<sharp> exp4"
-  shows "(var:== exp1 ; IF (qtop tp (VAR var) exp2 exp3 exp4) THEN C1 ELSE C2) = 
-         (IF (qtop tp exp1 exp2 exp3  exp4) THEN (var:== exp1 ; C1) ELSE (var:== exp1 ; C2))"
-  using 1 2 3 4 unfolding subst_upd_var_def unrest_def
-  by transfer auto
+lemma assign_cond_trop3:
+  assumes 1: "weak_lens v" and 2: "v \<sharp> exp2" and 3: "v \<sharp> exp3"
+  shows "(v:== exp1 ;; C1 \<triangleleft>(trop bp exp2 exp3 (&v))\<triangleright>\<^sub>r C2) = 
+         ((v:== exp1 ;; C1) \<triangleleft>(trop bp exp2 exp3 exp1)\<triangleright>\<^sub>r (v:== exp1 ;; C2))"
+  using 1 2 3 unfolding cond_def
+  by rel_auto
 
-lemma ASN11_qtop2:
-  assumes 1: "weak_lens var" and 2: "var \<sharp> exp2" and 3: "var \<sharp> exp3" and 4:"var \<sharp> exp4"
-  shows "(var:== exp1 ; IF (qtop tp exp2 (VAR var) exp3 exp4) THEN C1 ELSE C2) = 
-         (IF (qtop tp exp2 exp1 exp3 exp4) THEN (var:== exp1 ; C1) ELSE (var:== exp1 ; C2))"
-  using 1 2 3 4 unfolding subst_upd_var_def unrest_def
-  by transfer auto
+lemma assign_cond_qtop1:
+  assumes 1: "weak_lens v" and 2: "v \<sharp> exp2" and 3: "v \<sharp> exp3" and 4: "v \<sharp> exp4"
+  shows "(v:== exp1 ;;  C1 \<triangleleft>(qtop tp (&v) exp2 exp3 exp4)\<triangleright>\<^sub>r C2) = 
+         ((v:== exp1 ;; C1) \<triangleleft>(qtop tp exp1 exp2 exp3  exp4)\<triangleright>\<^sub>r (v:== exp1 ;; C2))"
+  using 1 2 3 4 unfolding cond_def
+  by rel_auto
 
-lemma ASN11_qtop3:
-  assumes 1: "weak_lens var" and 2: "var \<sharp> exp2" and 3: "var \<sharp> exp3" and 4: "var \<sharp> exp4"
-  shows "(var:== exp1 ; IF (qtop bp exp2 exp3 (VAR var) exp4) THEN C1 ELSE C2) = 
-         (IF (qtop bp exp2 exp3 exp1  exp4) THEN (var:== exp1 ; C1) ELSE (var:== exp1 ; C2))"
-  using 1 2 3 4 unfolding subst_upd_var_def unrest_def
-  by transfer auto
+lemma assign_cond_qtop2:
+  assumes 1: "weak_lens v" and 2: "v \<sharp> exp2" and 3: "v \<sharp> exp3" and 4:"v \<sharp> exp4"
+  shows "(v:== exp1 ;; C1 \<triangleleft>(qtop tp exp2 (&v) exp3 exp4)\<triangleright>\<^sub>r C2) = 
+         ((v:== exp1 ;; C1) \<triangleleft>(qtop tp exp2 exp1 exp3 exp4)\<triangleright>\<^sub>r  (v:== exp1 ;; C2))"
+  using 1 2 3 4 unfolding cond_def
+  by rel_auto
 
-lemma ASN11_qtop4:
-  assumes 1: "weak_lens var" and 2: "var \<sharp> exp2" and 3: "var \<sharp> exp3" and 4: "var \<sharp> exp4"
-  shows "(var:== exp1 ; IF (qtop bp exp2 exp3 exp4 (VAR var)) THEN C1 ELSE C2) = 
-         (IF (qtop bp exp2 exp3  exp4 exp1) THEN (var:== exp1 ; C1) ELSE (var:== exp1 ; C2))"
-  using 1 2 3 4 unfolding subst_upd_var_def unrest_def
-  by transfer auto
+lemma assign_cond_qtop3:
+  assumes 1: "weak_lens v" and 2: "v \<sharp> exp2" and 3: "v \<sharp> exp3" and 4: "v \<sharp> exp4"
+  shows "(v:== exp1 ;; C1 \<triangleleft>(qtop bp exp2 exp3 (&v) exp4)\<triangleright>\<^sub>r C2) = 
+         ((v:== exp1 ;; C1) \<triangleleft>(qtop bp exp2 exp3 exp1  exp4)\<triangleright>\<^sub>r (v:== exp1 ;; C2))"
+  using 1 2 3 4 unfolding cond_def
+  by rel_auto
 
-lemma ASN12[symbolic_exec_subst]:
-  "(IF bexp THEN (var:== exp1) ELSE (var:== exp2)) = 
-   (var :== (trop If bexp exp1 exp2))" 
-   unfolding subst_upd_var_def 
-   by transfer auto 
+lemma assign_cond_qtop4:
+  assumes 1: "weak_lens v" and 2: "v \<sharp> exp2" and 3: "v \<sharp> exp3" and 4: "v \<sharp> exp4"
+  shows "(v:== exp1 ;; C1 \<triangleleft>(qtop bp exp2 exp3 exp4 (&v))\<triangleright>\<^sub>r C2) = 
+         ((v:== exp1 ;; C1) \<triangleleft>(qtop bp exp2 exp3  exp4 exp1)\<triangleright>\<^sub>r (v:== exp1 ;; C2))"
+  using 1 2 3 4 unfolding cond_def
+  by rel_auto
 
-lemma ASN13_uop[symbolic_exec_subst]:
-  assumes 1: "mwb_lens var"
-  shows "((var:== E); 
-          IF uop F (VAR var) THEN (var:== (uop F (VAR var))) ELSE (var:== (uop G (VAR var)))) =
-         (var:== (trop If (uop F E) (uop F E) (uop G E)))" 
-  using 1 unfolding subst_upd_var_def 
-  by transfer auto
+lemma assign_cond_If [symbolic_exec_subst]:
+  "((v:== exp1) \<triangleleft> bexp\<triangleright>\<^sub>r (v:== exp2)) = 
+   (v :== (trop If bexp exp1 exp2))" 
+  unfolding cond_def
+  by rel_auto
 
-lemma ASN13_bop:
-  assumes 1: "mwb_lens var" and 2:"var \<sharp> exp"
-  shows "((var:== E); 
-          IF bop F exp (VAR var)  THEN (var:== (bop F exp (VAR var))) ELSE (var:== (bop G exp (VAR var)))) =
-         (var:== (trop If (bop F exp E) (bop F exp E) (bop G exp E)))" 
-  using 1 2 unfolding subst_upd_var_def unrest_def
-  by transfer auto
+lemma assign_cond_If_uop[symbolic_exec_subst]:
+  assumes 1: "mwb_lens v"
+  shows "(v:== E;; 
+         (v:== uop F (&v)) \<triangleleft>uop F (&v)\<triangleright>\<^sub>r (v:== uop G (&v))) =
+         (v:== trop If (uop F E) (uop F E) (uop G E))" 
+  using 1 unfolding cond_def
+  by rel_auto
 
-lemma ASN13_bop1:
-  assumes 1: "mwb_lens var" and 2:"var \<sharp> exp"
-  shows "((var:== E); 
-          IF bop F (VAR var) exp THEN (var:== (bop F (VAR var) exp)) ELSE (var:== (bop G (VAR var) exp))) =
-         (var:== (trop If (bop F E exp) (bop F E exp) (bop G E exp)))" 
-  using 1 2 unfolding subst_upd_var_def unrest_def
-  by transfer auto 
+lemma assign_cond_If_bop:
+  assumes 1: "mwb_lens v" and 2:"v \<sharp> exp"
+  shows "((v:== E);; 
+          (v:== (bop F exp (&v))) \<triangleleft>bop F exp (&v)\<triangleright>\<^sub>r (v:== (bop G exp (&v)))) =
+         (v:== (trop If (bop F exp E) (bop F exp E) (bop G exp E)))" 
+  using 1 2 unfolding cond_def
+  by rel_auto
 
-lemma ASN13_bop2:
-  assumes 1: "mwb_lens var" and 2:"var \<sharp> exp1" and 3:"var \<sharp> exp2"
-  shows "((var:== E); 
-          IF bop F (VAR var) exp1 THEN (var:== (bop F (VAR var) exp1)) ELSE (var:== (bop G (VAR var) exp2))) =
-         (var:== (trop If (bop F E exp1) (bop F E exp1) (bop G E exp2)))" 
-  using 1 2 3 unfolding subst_upd_var_def unrest_def
-  by transfer auto
+lemma assign_cond_If_bop1:
+  assumes 1: "mwb_lens v" and 2:"v \<sharp> exp"
+  shows "((v:== E);; 
+          (v:== (bop F (&v) exp)) \<triangleleft>bop F (&v) exp\<triangleright>\<^sub>r (v:== (bop G (&v) exp))) =
+         (v:== (trop If (bop F E exp) (bop F E exp) (bop G E exp)))" 
+  using 1 2 unfolding cond_def
+  by rel_auto
 
-lemma ASN13_bop3:
-  assumes 1: "mwb_lens var" and 2:"var \<sharp> exp"
-  shows "((var:== E); 
-          IF bop F exp (VAR var)  THEN (var:== (bop F exp (VAR var))) ELSE (var:== (bop G exp (VAR var)))) =
-         (var:== (trop If (bop F exp E) (bop F exp E) (bop G exp E)))" 
-  using 1 2 unfolding subst_upd_var_def unrest_def
-  by transfer auto
+lemma assign_cond_If_bop2:
+  assumes 1: "mwb_lens v" and 2:"v \<sharp> exp1" and 3:"v \<sharp> exp2"
+  shows "((v:== E);; 
+          (v:== (bop F (&v) exp1)) \<triangleleft>bop F (&v) exp1\<triangleright>\<^sub>r (v:== (bop G (&v) exp2))) =
+         (v:== (trop If (bop F E exp1) (bop F E exp1) (bop G E exp2)))" 
+  using 1 2 3 unfolding cond_def
+  by rel_auto
 
-lemma ASN13_bop4:
-  assumes 1: "mwb_lens var" and 2:"var \<sharp> exp1" and 3:"var \<sharp> exp2"
-  shows "((var:== E); 
-          IF bop F (VAR var) exp1 THEN (var:== (bop F (VAR var) exp1)) ELSE (var:== (bop G exp2 (VAR var)))) =
-         (var:== (trop If (bop F E exp1) (bop F E exp1) (bop G exp2 E)))" 
-  using 1 2 3 unfolding subst_upd_var_def unrest_def
-  by transfer auto
+lemma assign_cond_If_bop4:
+  assumes 1: "mwb_lens v" and 2:"v \<sharp> exp1" and 3:"v \<sharp> exp2"
+  shows "((v:== E);; 
+          (v:== (bop F (&v) exp1)) \<triangleleft>bop F (&v) exp1\<triangleright>\<^sub>r (v:== (bop G exp2 (&v)))) =
+         (v:== (trop If (bop F E exp1) (bop F E exp1) (bop G exp2 E)))" 
+  using 1 2 3 unfolding cond_def
+  by rel_auto
 
-lemma ASN13_bop5:
-  assumes 1: "mwb_lens var" and 2:"var \<sharp> exp1" and 3:"var \<sharp> exp2"
-  shows "((var:== E); 
-          IF bop F exp1 (VAR var) THEN (var:== (bop F exp1 (VAR var))) ELSE (var:== (bop G (VAR var) exp2))) =
-         (var:== (trop If (bop F exp1 E) (bop F exp1 E) (bop G E exp2)))" 
-  using 1 2 3 unfolding subst_upd_var_def unrest_def
-  by transfer auto
+lemma assign_cond_If_bop5:
+  assumes 1: "mwb_lens v" and 2:"v \<sharp> exp1" and 3:"v \<sharp> exp2"
+  shows "((v:== E);; 
+          (v:== (bop F exp1 (&v))) \<triangleleft>bop F exp1 (&v)\<triangleright>\<^sub>r (v:== (bop G (&v) exp2))) =
+         (v:== (trop If (bop F exp1 E) (bop F exp1 E) (bop G E exp2)))" 
+  using 1 2 3 unfolding cond_def
+  by rel_auto
 
-lemma ASN13_bop6:
-  assumes 1: "mwb_lens var" and 2:"var \<sharp> exp1" and 3:"var \<sharp> exp2"
-  shows "((var:== E); 
-          IF bop F exp1 (VAR var) THEN (var:== (bop F exp1 (VAR var))) ELSE (var:== (bop G exp2 (VAR var)))) =
-         (var:== (trop If (bop F exp1 E) (bop F exp1 E) (bop G exp2 E)))" 
-  using 1 2 3 unfolding subst_upd_var_def unrest_def
-  by transfer auto
+lemma assign_cond_If_bop6:
+  assumes 1: "mwb_lens v" and 2:"v \<sharp> exp1" and 3:"v \<sharp> exp2"
+  shows "((v:== E);; 
+          (v:== (bop F exp1 (&v))) \<triangleleft>bop F exp1 (&v)\<triangleright>\<^sub>r (v:== (bop G exp2 (&v)))) =
+         (v:== (trop If (bop F exp1 E) (bop F exp1 E) (bop G exp2 E)))" 
+  using 1 2 3 unfolding cond_def
+  by rel_auto
 
-lemma ASN13_trop:
-  assumes 1: "mwb_lens var" and 2:"var \<sharp> exp1" and 3:"var \<sharp> exp2"
-  shows "((var:== E); 
-          IF trop F exp1 exp2 (VAR var)  THEN (var:== (trop F exp1 exp2 (VAR var))) ELSE (var:== (trop G exp1 exp2 (VAR var)))) =
-         (var:== (trop If (trop F exp1 exp2 E) (trop F exp1 exp2 E) (trop G exp1 exp2 E)))" 
-  using 1 2 3 unfolding subst_upd_var_def unrest_def
-  by transfer auto
+lemma assign_cond_If_trop:
+  assumes 1: "mwb_lens v" and 2:"v \<sharp> exp1" and 3:"v \<sharp> exp2"
+  shows "((v:== E);;
+         (v:== (trop F exp1 exp2 (&v))) \<triangleleft>trop F exp1 exp2 (&v)\<triangleright>\<^sub>r (v:== (trop G exp1 exp2 (&v)))) =
+         (v:== (trop If (trop F exp1 exp2 E) (trop F exp1 exp2 E) (trop G exp1 exp2 E)))" 
+  using 1 2 3 unfolding cond_def
+  by rel_auto
 
-lemma ASN13_trop1:
-  assumes 1: "mwb_lens var" and 2:"var \<sharp> exp1" and 3:"var \<sharp> exp2"
-  shows "((var:== E); 
-          IF trop F exp1 (VAR var) exp2 THEN (var:== (trop F exp1 (VAR var) exp2)) ELSE (var:== (trop G exp1 (VAR var) exp2))) =
-         (var:== (trop If (trop F exp1 E exp2) (trop F exp1 E exp2) (trop G exp1 E exp2)))" 
-  using 1 2 3 unfolding subst_upd_var_def unrest_def
-  by transfer auto
+lemma assign_cond_If_trop1:
+  assumes 1: "mwb_lens v" and 2:"v \<sharp> exp1" and 3:"v \<sharp> exp2"
+  shows "((v:== E);; 
+          (v:== (trop F exp1 (&v) exp2)) \<triangleleft>trop F exp1 (&v) exp2\<triangleright>\<^sub>r (v:== (trop G exp1 (&v) exp2))) =
+         (v:== (trop If (trop F exp1 E exp2) (trop F exp1 E exp2) (trop G exp1 E exp2)))" 
+  using 1 2 3 unfolding cond_def
+  by rel_auto
 
-lemma ASN13_trop2:
-  assumes 1: "mwb_lens var" and 2:"var \<sharp> exp1" and 3:"var \<sharp> exp2"
-  shows "((var:== E); 
-          IF trop F (VAR var)  exp1 exp2 THEN (var:== (trop F (VAR var) exp1 exp2)) ELSE (var:== (trop G (VAR var)  exp1 exp2))) =
-         (var:== (trop If (trop F E exp1 exp2) (trop F E exp1 exp2) (trop G E exp1 exp2)))" 
-  using 1 2 3 unfolding subst_upd_var_def unrest_def
-  by transfer auto 
+lemma assign_cond_If_trop2:
+  assumes 1: "mwb_lens v" and 2:"v \<sharp> exp1" and 3:"v \<sharp> exp2"
+  shows "((v:== E);; 
+          (v:== (trop F (&v) exp1 exp2)) \<triangleleft>trop F (&v) exp1 exp2\<triangleright>\<^sub>r (v:== (trop G (&v) exp1 exp2))) =
+         (v:== (trop If (trop F E exp1 exp2) (trop F E exp1 exp2) (trop G E exp1 exp2)))" 
+  using 1 2 3 unfolding cond_def
+  by rel_auto
 
-lemma ASN13_trop3:
-  assumes 1: "mwb_lens var" and 2:"var \<sharp> exp1" and 3:"var \<sharp> exp2" and 4:"var \<sharp> exp3" and 5:"var \<sharp> exp4"
-  shows "((var:== E); 
-          IF trop F exp1 exp2 (VAR var) THEN (var:== (trop F exp1 exp2 (VAR var))) ELSE (var:== (trop G exp3 exp4 (VAR var)))) =
-         (var:== (trop If (trop F exp1 exp2 E) (trop F exp1 exp2 E) (trop G exp3 exp4 E)))" 
-  using 1 2 3 4 5 unfolding subst_upd_var_def unrest_def
-  by transfer auto
+lemma assign_cond_If_trop3:
+  assumes 1: "mwb_lens v" and 2:"v \<sharp> exp1" and 3:"v \<sharp> exp2" and 4:"v \<sharp> exp3" and 5:"v \<sharp> exp4"
+  shows "((v:== E);;
+          (v:== (trop F exp1 exp2 (&v))) \<triangleleft>trop F exp1 exp2 (&v)\<triangleright>\<^sub>r (v:== (trop G exp3 exp4 (&v)))) =
+         (v:== (trop If (trop F exp1 exp2 E) (trop F exp1 exp2 E) (trop G exp3 exp4 E)))" 
+  using 1 2 3 4 5 unfolding cond_def
+  by rel_auto
 
-lemma ASN13_trop4:
-  assumes 1: "mwb_lens var" and 2:"var \<sharp> exp1" and 3:"var \<sharp> exp2" and 4:"var \<sharp> exp3" and 5:"var \<sharp> exp4"
-  shows "((var:== E); 
-          IF trop F exp1 (VAR var) exp2 THEN (var:== (trop F exp1 (VAR var) exp2)) ELSE (var:== (trop G exp3 (VAR var) exp4))) =
-         (var:== (trop If (trop F exp1 E exp2) (trop F exp1 E exp2) (trop G exp3 E exp4)))" 
-  using 1 2 3 4 5 unfolding subst_upd_var_def unrest_def
-  by transfer auto
+lemma assign_cond_If_trop4:
+  assumes 1: "mwb_lens v" and 2:"v \<sharp> exp1" and 3:"v \<sharp> exp2" and 4:"v \<sharp> exp3" and 5:"v \<sharp> exp4"
+  shows "((v:== E);; 
+         (v:== (trop F exp1 (&v) exp2)) \<triangleleft>trop F exp1 (&v) exp2\<triangleright>\<^sub>r (v:== (trop G exp3 (&v) exp4))) =
+         (v:== (trop If (trop F exp1 E exp2) (trop F exp1 E exp2) (trop G exp3 E exp4)))" 
+  using 1 2 3 4 5 unfolding cond_def
+  by rel_auto
 
-lemma ASN13_trop5:
-  assumes 1: "mwb_lens var" and 2:"var \<sharp> exp1" and 3:"var \<sharp> exp2" and 4:"var \<sharp> exp3" and 5:"var \<sharp> exp4"
-  shows "((var:== E); 
-          IF trop F (VAR var) exp1 exp2 THEN (var:== (trop F (VAR var) exp1 exp2)) ELSE (var:== (trop G (VAR var) exp3 exp4))) =
-         (var:== (trop If (trop F E exp1 exp2) (trop F E exp1 exp2) (trop G E exp3 exp4)))" 
-  using 1 2 3 4 5 unfolding subst_upd_var_def unrest_def
-  by transfer auto
-
-theorem ASN14:
-  assumes "mwb_lens x" and "x \<sharp>\<sharp> \<guillemotleft>SOME \<sigma>. True\<guillemotright>"
-  shows
-  "((IF b THEN x :== E ELSE \<guillemotleft>SOME \<sigma>. True\<guillemotright>); 
-    (IF (uop c (VAR x)) THEN (x :== (uop F (VAR x))) ELSE \<guillemotleft>SOME \<sigma>. True\<guillemotright> )) = 
-    (IF (trop If b (uop c  E) \<guillemotleft>False\<guillemotright>) THEN x :== (uop F E) ELSE \<guillemotleft>SOME \<sigma>. True\<guillemotright>)"
-  using assms unfolding unrest_usubst_def subst_upd_var_def   
-  by transfer auto 
-
-theorem ASN15:
-  assumes "mwb_lens x" and "x \<sharp>\<sharp> \<guillemotleft>bot\<guillemotright>"
-  shows
-  "((IF b THEN x :== E ELSE \<guillemotleft>bot\<guillemotright>); 
-    (IF (uop c (VAR x)) THEN (x :== (uop F (VAR x))) ELSE \<guillemotleft>bot\<guillemotright> )) = 
-    (IF (trop If b (uop c  E) \<guillemotleft>False\<guillemotright>) THEN x :== (uop F E) ELSE \<guillemotleft>bot\<guillemotright>)"
-  using assms unfolding unrest_usubst_def subst_upd_var_def   
-  by transfer auto
+lemma assign_cond_If_trop5:
+  assumes 1: "mwb_lens v" and 2:"v \<sharp> exp1" and 3:"v \<sharp> exp2" and 4:"v \<sharp> exp3" and 5:"v \<sharp> exp4"
+  shows "((v:== E);; 
+          (v:== (trop F (&v) exp1 exp2)) \<triangleleft>trop F (&v) exp1 exp2\<triangleright>\<^sub>r (v:== (trop G (&v) exp3 exp4))) =
+         (v:== (trop If (trop F E exp1 exp2) (trop F E exp1 exp2) (trop G E exp3 exp4)))" 
+  using 1 2 3 4 5 unfolding cond_def
+  by rel_auto
 
 subsection {*Conditional Laws*}
 text{*In this section we introduce the algebraic laws of programming related to the conditional
       statement.*}
- 
-(*IF True*)
-lemma COND1[symbolic_exec_subst]:
-  "(IF TRUE THEN C1 ELSE C2) = C1" 
-  by transfer simp
 
-(*IF False*)
-lemma COND2[symbolic_exec_subst]:
-  "(IF FALSE THEN C1 ELSE C2) = C2" 
-  by transfer simp
+lemma cond_idem[symbolic_exec_subst]:
+  "(IF b THEN P ELSE P) = P" 
+  unfolding cond_def by rel_auto
 
-(*IF Idemp*)
-lemma COND3[symbolic_exec_subst]:
-  "(IF bexp THEN C1 ELSE C1) = C1" 
-  by simp
+lemma cond_symm:
+  "(IF b THEN P ELSE Q) = (IF \<not> b THEN Q ELSE P)" 
+  unfolding cond_def by rel_auto
 
-(*IF assoc*)
-lemma COND4:
-  "(IF bexp THEN C1 ELSE (IF bexp THEN C2 ELSE C3)) =  
-   (IF bexp THEN (IF bexp THEN C1 ELSE C2) ELSE C3)" 
-  by auto
+lemma cond_assoc: 
+  "(IF b THEN P ELSE (IF b THEN Q ELSE R)) =  
+   (IF b THEN (IF b THEN P ELSE Q) ELSE R)"  
+   unfolding cond_def by rel_auto
 
-(*IF inverse*)
-lemma COND5:
-  "(IF P THEN C1 ELSE C2) = (IF \<not>\<^sub>e P THEN C2 ELSE C1)" 
-  by transfer auto
+lemma cond_distr[symbolic_exec_subst]: 
+  "(IF b THEN (IF b' THEN P ELSE R) ELSE (IF b' THEN Q ELSE R))=  
+   (IF b' THEN (IF b THEN P ELSE Q) ELSE R)" 
+  unfolding cond_def by rel_auto
 
-(*IF unfold nested cond*)
-lemma COND6[symbolic_exec_subst]:
-  "(IF bexp THEN (IF bexp1 THEN C1 ELSE C2) ELSE (IF bexp2 THEN C1 ELSE C2)) = 
-   (IF trop If bexp bexp1 bexp2 THEN C1 ELSE C2)" 
-  by transfer auto
+lemma cond_unit_T [simp, symbolic_exec_subst]:"(IF true THEN P ELSE Q) = P" 
+  unfolding cond_def by rel_auto
 
-(*IF ignore*)
-lemma COND7[symbolic_exec_subst]:
-  "(IF bexp THEN C1 ELSE (IF bexp THEN C2 ELSE C3)) = 
-   (IF bexp THEN C1 ELSE C3)" 
-  by auto
+lemma cond_unit_F [simp, symbolic_exec_subst]:"(IF false THEN P ELSE Q) = Q" 
+  unfolding cond_def by rel_auto
 
-(*the rules COND8, COND9 and COND10 are related to non-deterministic choice between C1 and C2..
-  which is not yet supported by our language*)
+lemma cond_and_T_integrate[symbolic_exec_subst]:
+  "((P \<and> b) \<or> (IF b THEN Q ELSE R)) = (IF b THEN (P \<or> Q) ELSE R)"
+  unfolding cond_def by rel_auto
 
-(*IF distribute*)
-lemma COND11[symbolic_exec_subst]:
-  "(IF bexp1 THEN (IF bexp2 THEN C1 ELSE C3) ELSE (IF bexp2 THEN C2 ELSE C3))=  
-   (IF bexp2 THEN (IF bexp1 THEN C1 ELSE C2) ELSE C3)" 
-  by auto
+lemma cond_L6[symbolic_exec_subst]: 
+  "(IF b THEN P ELSE (IF b THEN Q ELSE R)) = 
+   (IF b THEN P ELSE R)" 
+  unfolding cond_def by rel_auto
+
+lemma cond_L7[symbolic_exec_subst]: 
+  "(IF b THEN P ELSE (IF c THEN P ELSE Q)) = 
+   (IF b \<or> c THEN P ELSE Q)"
+  unfolding cond_def by rel_auto
+
+lemma cond_and_distr[symbolic_exec_subst]: 
+  "(IF b THEN (P \<and> Q) ELSE (R \<and> S)) = 
+   ((IF b THEN P ELSE R) \<and> (IF b THEN Q ELSE S))"  
+  unfolding cond_def by rel_auto
+
+lemma cond_or_distr[symbolic_exec_subst]: 
+  "(IF b THEN (P \<or> Q) ELSE (R \<or> S)) = 
+   ((IF b THEN P ELSE R) \<or> (IF b THEN Q ELSE S))" 
+  unfolding cond_def by rel_auto
+
+lemma cond_imp_distr[symbolic_exec_subst]:
+  "(IF b THEN (P \<Rightarrow> Q) ELSE (R \<Rightarrow> S)) = 
+   ((IF b THEN P ELSE R) \<Rightarrow> (IF b THEN Q ELSE S))" 
+  unfolding cond_def by rel_auto
+
+lemma cond_eq_distr[symbolic_exec_subst]:
+  "(IF b THEN (P \<Leftrightarrow> Q) ELSE (R \<Leftrightarrow> S)) = 
+   ((IF b THEN P ELSE R) \<Leftrightarrow> (IF b THEN Q ELSE S))"
+  unfolding cond_def by rel_auto
+
+lemma cond_conj_distr[symbolic_exec_subst]:
+  "(P \<and> (IF b THEN Q ELSE S)) = (IF b THEN (P \<and> Q) ELSE (P \<and> S))"  
+  unfolding cond_def by rel_auto
+
+lemma cond_disj_distr [symbolic_exec_subst]:
+  "(P \<or> (IF b THEN Q ELSE S)) = (IF b THEN (P \<or> Q) ELSE (P \<or> S))" 
+  unfolding cond_def by rel_auto 
+
+lemma cond_neg[symbolic_exec_subst]: 
+  "\<not> (IF b THEN P ELSE Q) = (IF b THEN (\<not> P) ELSE (\<not> Q))"
+  unfolding cond_def by rel_auto 
+
+(*lemma cond_USUP_dist: 
+  "IF b THEN (\<Squnion> P\<in>S \<bullet> F(P)) ELSE (\<Squnion> P\<in>S \<bullet> G(P)) = (IF b THEN \<Squnion> P\<in>S \<bullet> F(P) ELSE G(P))"
+  by (subst uexpr_eq_iff, auto simp add: disj_upred_def conj_upred_def not_upred_def cond_def UINF.rep_eq uminus_uexpr_def inf_uexpr.rep_eq sup_uexpr.rep_eq uop.rep_eq bop.rep_eq lit.rep_eq)
+
+lemma cond_UINF_dist: "(\<Sqinter> P\<in>S \<bullet> F(P)) \<triangleleft> b \<triangleright> (\<Sqinter> P\<in>S \<bullet> G(P)) = (\<Sqinter> P\<in>S \<bullet> F(P) \<triangleleft> b \<triangleright> G(P))"
+  by (subst uexpr_eq_iff, auto simp add: disj_upred_def conj_upred_def not_upred_def cond_def USUP.rep_eq uminus_uexpr_def inf_uexpr.rep_eq sup_uexpr.rep_eq uop.rep_eq bop.rep_eq lit.rep_eq)
+*)
+
+lemma cond_conj[symbolic_exec_subst]: 
+  "(IF b \<and> c THEN P ELSE Q) = IF b THEN (IF c THEN P ELSE Q) ELSE Q"
+  unfolding cond_def by rel_auto 
+    
 
 (*IF Theorem by Hoare: It optimize nested IF*)
 theorem COND12[symbolic_exec_subst]: 
   "(IF bexp1 THEN (IF bexp2 THEN C1 ELSE C3) ELSE (IF bexp3 THEN C2 ELSE C3)) =
    (IF (trop If bexp1 bexp2 bexp3) THEN (IF bexp1 THEN C1 ELSE C2) ELSE C3)"
-  by transfer auto
+  unfolding cond_def by rel_auto 
+ 
+lemma comp_cond_left_distr:
+  "((P \<triangleleft> b \<triangleright>\<^sub>r Q) ;; R) = ((P ;; R) \<triangleleft> b \<triangleright>\<^sub>r (Q ;; R))"
+  unfolding cond_def by rel_auto
+ 
+lemma cond_var_subst_left:
+  assumes "vwb_lens x"
+  shows "(IF &x THEN P\<lbrakk>true/x\<rbrakk> ELSE Q) = (IF  &x THEN P ELSE Q)"
+  using assms
+  by (metis cond_def conj_var_subst pr_var_def upred_eq_true utp_pred.inf.commute)
 
-lemma COND13:
-  assumes 1: "\<lceil>bexp\<rceil>"
-  shows 
-  "(IF bexp THEN C1 ELSE C2)=  C1"
-  using 1 
-  by transfer auto
+lemma cond_var_subst_right:
+  assumes "vwb_lens x"
+  shows "(IF &x THEN P ELSE Q\<lbrakk>false/x\<rbrakk>) = (IF &x THEN P ELSE Q)"
+  using assms
+  by (metis cond_def  conj_var_subst pr_var_def upred_eq_false utp_pred.inf.commute)
 
-lemma COND14:
-  assumes 1: "\<lceil>\<not>\<^sub>e bexp\<rceil>"
-  shows 
-  "(IF bexp THEN C1 ELSE C2)=  C2"
-  using 1 
-  by transfer auto
+
+lemma cond_var_split:
+  "vwb_lens x \<Longrightarrow> (IF &x THEN P\<lbrakk>true/x\<rbrakk> ELSE P\<lbrakk>false/x\<rbrakk>) = P"
+  unfolding cond_def
+  by (rel_auto, (metis (full_types) vwb_lens.put_eq)+)
+
+lemma cond_seq_left_distr:
+  "out\<alpha> \<sharp> b \<Longrightarrow> ((IF b THEN P ELSE Q) ;; R) = (IF b THEN (P ;; R) ELSE (Q ;; R))"
+   unfolding cond_def
+   by rel_auto
+
+lemma cond_seq_right_distr:
+  "in\<alpha> \<sharp> b \<Longrightarrow> (P ;; (IF b THEN Q ELSE R)) = (IF b THEN (P ;; Q) ELSE (P ;; R))"
+  unfolding cond_def
+  by rel_auto
 
 subsection {*Sequential Laws*}
 text{*In this section we introduce the algebraic laws of programming related to the sequential
       composition of statements.*}
 
-(*Seq assoc*)
-lemma SEQ1: 
-  "(C1 ; C2) ; C3 = C1 ; (C2 ; C3)"
-  by auto
+
+lemma seqr_exists_left: (*legacy: mwb_lens x \<Longrightarrow>*)
+  "((\<exists> $x \<bullet> P) ;; Q) = (\<exists> $x \<bullet> (P ;; Q))"
+  by (rel_auto)
+
+lemma seqr_exists_right: (*legacy: mwb_lens x \<Longrightarrow>*)
+  "(P ;; (\<exists> $x\<acute> \<bullet> Q)) = (\<exists> $x\<acute> \<bullet> (P ;; Q))"
+  by (rel_auto)
+
+lemma seqr_left_zero [simp, symbolic_exec_subst]:
+  "false ;; P = false"
+  by pred_auto
+
+lemma seqr_right_zero [simp, symbolic_exec_subst]:
+  "P ;; false = false"
+  by pred_auto
+
+lemma seqr_assoc: "P ;; (Q ;; R) = (P ;; Q) ;; R"
+  by rel_auto
+
+lemma seqr_or_distl:
+  "((P \<or> Q) ;; R) = ((P ;; R) \<or> (Q ;; R))"
+  by rel_auto
+
+lemma seqr_or_distr:
+  "(P ;; (Q \<or> R)) = ((P ;; Q) \<or> (P ;; R))"
+  by rel_auto
+
+lemma seqr_unfold:
+  "(P ;; Q) = (\<^bold>\<exists> v \<bullet> P\<lbrakk>\<guillemotleft>v\<guillemotright>/$\<Sigma>\<acute>\<rbrakk> \<and> Q\<lbrakk>\<guillemotleft>v\<guillemotright>/$\<Sigma>\<rbrakk>)"
+  by rel_auto
+
+lemma seqr_middle:
+  assumes "vwb_lens x"
+  shows "(P ;; Q) = (\<^bold>\<exists> v \<bullet> P\<lbrakk>\<guillemotleft>v\<guillemotright>/$x\<acute>\<rbrakk> ;; Q\<lbrakk>\<guillemotleft>v\<guillemotright>/$x\<rbrakk>)"
+  using assms
+  apply (rel_auto)
+  apply (rename_tac xa P Q a b y)
+  apply (rule_tac x="get\<^bsub>xa\<^esub> y" in exI)
+  apply (rule_tac x="y" in exI)
+  apply (simp)
+done
+
+lemma seqr_left_one_point:
+  assumes "vwb_lens x"
+  shows "((P \<and> $x\<acute> =\<^sub>u \<guillemotleft>v\<guillemotright>) ;; Q) = (P\<lbrakk>\<guillemotleft>v\<guillemotright>/$x\<acute>\<rbrakk> ;; Q\<lbrakk>\<guillemotleft>v\<guillemotright>/$x\<rbrakk>)"
+  using assms
+  by (rel_auto, metis vwb_lens_wb wb_lens.get_put)
+
+lemma seqr_right_one_point:
+  assumes "vwb_lens x"
+  shows "(P ;; ($x =\<^sub>u \<guillemotleft>v\<guillemotright> \<and> Q)) = (P\<lbrakk>\<guillemotleft>v\<guillemotright>/$x\<acute>\<rbrakk> ;; Q\<lbrakk>\<guillemotleft>v\<guillemotright>/$x\<rbrakk>)"
+  using assms
+  by (rel_auto, metis vwb_lens_wb wb_lens.get_put)
+
+lemma seqr_insert_ident_left:
+  assumes "vwb_lens x" "$x\<acute> \<sharp> P" "$x \<sharp> Q"
+  shows "(($x\<acute> =\<^sub>u $x \<and> P) ;; Q) = (P ;; Q)"
+  using assms
+  by (rel_auto, meson vwb_lens_wb wb_lens_weak weak_lens.put_get)
+
+lemma seqr_insert_ident_right:
+  assumes "vwb_lens x" "$x\<acute> \<sharp> P" "$x \<sharp> Q"
+  shows "(P ;; ($x\<acute> =\<^sub>u $x \<and> Q)) = (P ;; Q)"
+  using assms
+  by (rel_auto, metis (no_types, hide_lams) vwb_lens_def wb_lens_def weak_lens.put_get)
+
+lemma seq_var_ident_lift:
+  assumes "vwb_lens x" "$x\<acute> \<sharp> P" "$x \<sharp> Q"
+  shows "(($x\<acute> =\<^sub>u $x \<and> P) ;; ($x\<acute> =\<^sub>u $x \<and> Q)) = ($x\<acute> =\<^sub>u $x \<and> (P ;; Q))"
+  using assms apply (rel_auto)
+  by (metis (no_types, lifting) vwb_lens_wb wb_lens_weak weak_lens.put_get)
 
 (*Seq SKIP*)
-lemma SEQ2: 
-  "(SKIP ; C) = (C ; SKIP)"
+lemma seqr_skip: 
+  "(SKIP ;; C) = (C ;; SKIP)"
   by transfer simp
-
-(*Seq unit 1*)
-lemma SEQ3: 
-  "((0\<^sub>L :== VAR 0\<^sub>L) ; C) = (C ; (0\<^sub>L :== VAR 0\<^sub>L))"
-  unfolding subst_upd_var_def unit_lens_def
-  by transfer auto
-
-lemma SEQ4: 
-  "(bot ; C) = (C ; bot)"
-  unfolding subst_upd_var_def unit_lens_def
- oops
-
-(*Seq unit 2*)
-
-lemma SEQ5: 
-  "(bot ; C) = bot" 
-oops
-
-(*Seq unit 3*)
-lemma SEQ6: 
-  "(C ; bot) = bot"
-  by auto
 
 (*The rules SEQ6 SEQ7 related to SEQ and non-deterministic choice are missing for now*)
   
-(*Seq distribution*)
-lemma SEQ7[symbolic_exec_subst]: 
-  "(IF bexp THEN (C1 ; C3) ELSE (C2 ; C3))= 
-   ((IF bexp THEN C1 ELSE C2); C3)"
-   by transfer auto 
-
 subsection {*While laws*}
 text{*In this section we introduce the algebraic laws of programming related to the while
       statement.*}
 
-lemma W_mono: "mono (W b r)"
-  unfolding W_def mono_def
-  by auto
-
-
-(* A little complete partial order theory due to Tobias Nipkow, see also IMP as well as 
-   Monads-theory. *)
-definition chain :: "(nat \<Rightarrow> 'a set) \<Rightarrow> bool" 
-where     "chain S = (\<forall>i. S i \<subseteq> S(Suc i))"
-
-lemma chain_total: "chain S \<Longrightarrow> S i \<le> S j \<or> S j \<le> S i"
-by (metis chain_def le_cases lift_Suc_mono_le)
-
-definition cont :: "('a set \<Rightarrow> 'b set) \<Rightarrow> bool" 
-where     "cont f = (\<forall>S. chain S \<longrightarrow> f(UN n. S n) = (UN n. f(S n)))"
-
-lemma mono_if_cont: fixes f :: "'a set => 'b set"
-  assumes "cont f" shows "mono f"
-proof
-  fix a b :: "'a set" assume "a \<subseteq> b"
-  let ?S = "\<lambda>n::nat. if n=0 then a else b"
-  have "chain ?S" using `a \<subseteq> b` by(auto simp: chain_def)
-  hence "f(UN n. ?S n) = (UN n. f(?S n))"
-    using assms by(simp add: cont_def)
-  moreover have "(UN n. ?S n) = b" using `a \<subseteq> b` by (auto split: if_splits)
-  moreover have "(UN n. f(?S n)) = f a \<union> f b" by (auto split: if_splits)
-  ultimately show "f a \<subseteq> f b" by (metis Un_upper1)
+theorem while_unfold:
+  "WHILE b DO P OD = ((P ;; WHILE b DO P OD) \<triangleleft> b \<triangleright>\<^sub>r SKIP)"
+proof -
+  have m:"mono (\<lambda>X. (P ;; X) \<triangleleft> b \<triangleright>\<^sub>r SKIP)"
+    by (auto intro: monoI seqr_mono cond_mono)
+  have "(WHILE b DO P OD) = (\<nu> X \<bullet> (P ;; X) \<triangleleft> b \<triangleright>\<^sub>r SKIP)"
+    by (simp add: While_def)
+  also have "... = ((P ;; (\<nu> X \<bullet> (P ;; X) \<triangleleft> b \<triangleright>\<^sub>r SKIP)) \<triangleleft> b \<triangleright>\<^sub>r SKIP)"
+    by (subst lfp_unfold, simp_all add: m)
+  also have "... = ((P ;; WHILE b DO P OD) \<triangleleft> b \<triangleright>\<^sub>r SKIP)"
+    by (simp add: While_def)
+  finally show ?thesis .
 qed
 
-lemma chain_iterates: fixes f :: "'a set \<Rightarrow> 'a set"
-  assumes "mono f" shows "chain(\<lambda>n. (f^^n) {})"
-proof-
-  { fix n have "(f ^^ n) {} \<subseteq> (f ^^ Suc n) {}" using assms
-    by(induction n) (auto simp: mono_def) }
-  thus ?thesis by(auto simp: chain_def)
+lemma while_true:
+  assumes 1:"b = true"
+  shows "(WHILE b DO P OD) = (P ;; WHILE b DO P OD)"
+proof -
+  have "(WHILE b DO P OD) = (P ;; WHILE b DO P OD) \<triangleleft> b \<triangleright>\<^sub>r SKIP" 
+    using while_unfold[of b P] by simp
+  also have "... = (P ;; WHILE b DO P OD)" 
+    using 1 by (simp add: aext_true)
+  finally show ?thesis .
 qed
 
-theorem lfp_if_cont:
-  assumes "cont f" shows "lfp f = (UN n. (f^^n) {})" (is "_ = ?U")
-proof
-  show "lfp f \<subseteq> ?U"
-  proof (rule lfp_lowerbound)
-    have "f ?U = (UN n. (f^^Suc n){})"
-      using chain_iterates[OF mono_if_cont[OF assms]] assms
-      by(simp add: cont_def)
-    also have "\<dots> = (f^^0){} \<union> \<dots>" by simp
-    also have "\<dots> = ?U"
-      by(auto simp del: funpow.simps) (metis not0_implies_Suc)
-    finally show "f ?U \<subseteq> ?U" by simp
-  qed
-next
-  { fix n p assume "f p \<subseteq> p"
-    have "(f^^n){} \<subseteq> p"
-    proof(induction n)
-      case 0 show ?case by simp
-    next
-      case Suc
-      from monoD[OF mono_if_cont[OF assms] Suc] `f p \<subseteq> p`
-      show ?case by simp
-    qed
-  }
-  thus "?U \<subseteq> lfp f" by(auto simp: lfp_def)
+lemma while_false:
+  assumes 1:"b = false"
+  shows "(WHILE b DO P OD) = SKIP"
+proof -
+  have "(WHILE b DO P OD) = (P ;; WHILE b DO P OD) \<triangleleft> b \<triangleright>\<^sub>r SKIP" 
+    using while_unfold[of b P] by simp
+  also have "... = SKIP" 
+    using 1 by (simp add: aext_false)
+  finally show ?thesis . 
 qed
-
-
-lemma single_valued_UN_chain:
-  assumes "chain S" "(!!n. single_valued (S n))"
-  shows "single_valued(UN n. S n)"
-proof(auto simp: single_valued_def)
-  fix m n x y z assume "(x, y) \<in> S m" "(x, z) \<in> S n"
-  with chain_total[OF assms(1), of m n] assms(2)
-  show "y = z" by (auto simp: single_valued_def)
-qed
-
-lemma single_valued_lfp: 
-fixes f :: "('a \<times> 'a) set \<Rightarrow> ('a \<times> 'a) set"
-assumes "cont f" "\<And>r. single_valued r \<Longrightarrow> single_valued (f r)"
-shows "single_valued(lfp f)"
-unfolding lfp_if_cont[OF assms(1)]
-proof(rule single_valued_UN_chain[OF chain_iterates[OF mono_if_cont[OF assms(1)]]])
-  fix n show "single_valued ((f ^^ n) {})"
-  by(induction n)(auto simp: assms(2))
-qed
-
-lemma cont_W: "cont (W c b)"
-  by (auto simp: cont_def W_def)
-
-theorem single_valued_lfp_Fun2Rel: "single_valued (lfp(W c (Rel B)))"
-  apply(rule single_valued_lfp, simp_all add: cont_W)
-  apply(auto simp: W_def single_valued_def)
-  apply (simp add: Commands.Rel_def)
-done
-
-lemma Rel2Fun_if:
-  "RelInv {(s, t). if b s then (s, t) \<in> Rel c O lfp (W b (Rel c)) else s = t} \<sigma> =
-  (if b \<sigma> then RelInv (Rel c O lfp (W b (Rel c))) \<sigma> else  \<sigma>)"
-  by (simp add: RelInv_def)
-
-
-lemma Rel2Fun_Id: "(RelInv \<circ> Rel) x = x"
-  by (rule ext, auto simp: comp_def Rel_def RelInv_def)
-
-lemma Rel2Fun_homomorphism:
-  assumes determ_X: "single_valued X" and determ_Y: "single_valued Y"
-          and "is_total X" and "is_total Y"
-  shows   "RelInv (X O Y) = (RelInv Y) o (RelInv X)"
-proof - 
-    have relational_partial_next_in_O: 
-         "\<And>x E F. (\<exists>y. (x, y) \<in> (E O F)) \<Longrightarrow> (\<exists>y. (x, y) \<in> E)" by auto
-    have some_eq_intro:
-         "\<And> Z x y . single_valued Z \<Longrightarrow> (x, y) \<in> Z \<Longrightarrow> (SOME y. (x, y) \<in> Z) = y"
-          by (auto simp: single_valued_def)
-    show ?thesis
-    proof (rule ext, rename_tac "\<sigma>", simp add: RelInv_def)?
-     fix \<sigma> :: 'a
-     { fix aa :: 'a
-       obtain aaa :: "('a \<Rightarrow> 'a \<Rightarrow> bool) \<Rightarrow> ('a \<Rightarrow> 'a \<Rightarrow> bool) \<Rightarrow> 'a \<Rightarrow> 'a \<Rightarrow> 'a" where
-         ff1: "\<forall>p pa a aa. (\<not> (p OO pa) a aa \<or> p a (aaa p pa a aa) \<and> pa (aaa p pa a aa) aa) \<and> ((\<forall>ab. \<not> p a ab \<or> \<not> pa ab aa) \<or> (p OO pa) a aa)"
-         by moura
-       { assume "(SOME a. (\<sigma>, a) \<in> X, aa) \<notin> Y"
-         moreover
-         { assume "(aaa (\<lambda>a aa. (a, aa) \<in> X) (\<lambda>a aa. (a, aa) \<in> Y) \<sigma> aa, aa) \<notin> Y \<and> (SOME a. (\<sigma>, a) \<in> X, aa) \<notin> Y"
-           then have "\<not> ((\<lambda>a aa. (a, aa) \<in> X) OO (\<lambda>a aa. (a, aa) \<in> Y)) \<sigma> aa \<and> (SOME a. (\<sigma>, a) \<in> X, aa) \<notin> Y"
-             using ff1 by meson }
-         ultimately have "(\<sigma>, SOME a. (\<sigma>, a) \<in> X) \<in> X \<longrightarrow> ((SOME a. (\<sigma>, a) \<in> X O Y) = (SOME a. (SOME a. (\<sigma>, a) \<in> X, a) \<in> Y) \<or> (\<sigma>, aa) \<notin> X O Y \<and> (SOME a. (\<sigma>, a) \<in> X, aa) \<notin> Y \<or> (\<sigma>, aa) \<in> X O Y \<and> (SOME a. (\<sigma>, a) \<in> X, aa) \<in> Y) \<or> \<not> ((\<lambda>a aa. (a, aa) \<in> X) OO (\<lambda>a aa. (a, aa) \<in> Y)) \<sigma> aa \<and> (SOME a. (\<sigma>, a) \<in> X, aa) \<notin> Y \<or> (\<sigma>, aaa (\<lambda>a aa. (a, aa) \<in> X) (\<lambda>a aa. (a, aa) \<in> Y) \<sigma> aa) \<notin> X \<and> (SOME a. (\<sigma>, a) \<in> X, aa) \<notin> Y \<or> \<not> ((\<lambda>a aa. (a, aa) \<in> X) OO (\<lambda>a aa. (a, aa) \<in> Y)) \<sigma> aa \<and> (\<sigma>, aa) \<notin> X O Y"
-           by (metis (lifting) determ_X some_eq_intro) }
-       moreover
-       { assume "(\<sigma>, SOME a. (\<sigma>, a) \<in> X) \<notin> X"
-         moreover
-         { assume "\<exists>a. \<not> ((\<lambda>a aa. (a, aa) \<in> X) OO (\<lambda>a aa. (a, aa) \<in> Y)) \<sigma> aa \<and> (\<sigma>, aa) \<notin> X O Y \<and> (\<sigma>, a) \<in> X"
-           then have "\<exists>a p. p (a::'a) (SOME a. (\<sigma>, a) \<in> X) \<and> \<not> (p OO (\<lambda>a aa. (a, aa) \<in> Y)) a aa \<and> (\<sigma>, aa) \<notin> X O Y"
-             by (meson exE_some) }
-         ultimately have "(\<sigma>, aa) \<in> X O Y \<and> (\<sigma>, SOME a. (\<sigma>, a) \<in> X) \<notin> X \<or> (\<exists>a p. p (a::'a) (SOME a. (\<sigma>, a) \<in> X) \<and> \<not> (p OO (\<lambda>a aa. (a, aa) \<in> Y)) a aa \<and> (\<sigma>, aa) \<notin> X O Y)"
-           by (metis (no_types) assms(3) is_total_def relcompp_relcomp_eq)
-         then have "(\<exists>a p. p (a::'a) (SOME a. (\<sigma>, a) \<in> X) \<and> \<not> (p OO (\<lambda>a aa. (a, aa) \<in> Y)) a aa \<and> (\<sigma>, aa) \<notin> X O Y) \<or> (\<sigma>, aaa (\<lambda>a aa. (a, aa) \<in> X) (\<lambda>a aa. (a, aa) \<in> Y) \<sigma> aa) \<notin> X \<and> (SOME a. (\<sigma>, a) \<in> X, aa) \<notin> Y \<or> (SOME a. (\<sigma>, a) \<in> X O Y) = (SOME a. (SOME a. (\<sigma>, a) \<in> X, a) \<in> Y) \<or> (\<sigma>, aa) \<notin> X O Y \<and> (SOME a. (\<sigma>, a) \<in> X, aa) \<notin> Y \<or> (\<sigma>, aa) \<in> X O Y \<and> (SOME a. (\<sigma>, a) \<in> X, aa) \<in> Y"
-           by (meson exE_some) }
-       moreover
-       { assume "(\<sigma>, aaa (\<lambda>a aa. (a, aa) \<in> X) (\<lambda>a aa. (a, aa) \<in> Y) \<sigma> aa) \<notin> X \<and> (SOME a. (\<sigma>, a) \<in> X, aa) \<notin> Y"
-         then have "\<not> ((\<lambda>a aa. (a, aa) \<in> X) OO (\<lambda>a aa. (a, aa) \<in> Y)) \<sigma> aa \<and> (SOME a. (\<sigma>, a) \<in> X, aa) \<notin> Y"
-           using ff1 by meson }
-       ultimately have "(SOME a. (\<sigma>, a) \<in> X O Y) = (SOME a. (SOME a. (\<sigma>, a) \<in> X, a) \<in> Y) \<or> (\<sigma>, aa) \<notin> X O Y \<and> (SOME a. (\<sigma>, a) \<in> X, aa) \<notin> Y \<or> (\<sigma>, aa) \<in> X O Y \<and> (SOME a. (\<sigma>, a) \<in> X, aa) \<in> Y"
-         by blast }
-     then show "(SOME a. (\<sigma>, a) \<in> X O Y) = (SOME a. (SOME a. (\<sigma>, a) \<in> X, a) \<in> Y)"
-       by meson
-   qed
-qed
-
-(*apply (case_tac " \<exists> \<sigma>'. (\<sigma>, \<sigma>') \<in> X O Y")
-apply (simp )
-apply (frule relational_partial_next_in_O)
-apply (auto simp: single_valued_relcomp some_eq_intro determ_X determ_Y relcomp.relcompI)
-by (meson assms(3) assms(4) is_total_def relcomp.relcompI)*)
-
-lemma single_valued_Rel: "single_valued (Rel B)"
-by (auto simp: single_valued_def Rel_def)
-
-
-text{* Putting everything together, the theory of embedding and the invariant of
-       determinism of the while-body, gives us the usual unfold-theorem: *}
-
-theorem WHILE_unfold:
-assumes loop_terminates: "is_total (lfp (W b (Rel c)))"
-shows  "(WHILE b DO c OD) = (IF b THEN (c ; (WHILE b DO c OD)) ELSE SKIP)"
-proof (rule ext)
-  fix \<sigma>
-  have h1:"(WHILE b DO c OD) = RelInv (W b (Rel c) (lfp (W b (Rel c)))) "
-    using lfp_unfold [OF mono_if_cont, OF cont_W, of b "Rel c"]
-    unfolding While_def
-    by simp
-  show "(WHILE b DO c OD) \<sigma> =
-         (IF b THEN c; WHILE b DO c OD ELSE SKIP) \<sigma>"
-   by (subst h1, subst W_def) 
-      (auto simp: While_def h1 Rel2Fun_if Rel2Fun_homomorphism  Rel2Fun_Id [simplified comp_def] 
-                  single_valued_Rel  single_valued_lfp_Fun2Rel loop_terminates)
-qed
-
-lemma WHILE_True:
-  assumes 1:"\<lceil>b\<rceil>" and 2:"is_total (lfp (W b (Rel c)))" 
-  shows "(WHILE b DO c OD) = (c; WHILE b DO c OD)"
-  using 1  2
-  by (subst WHILE_unfold) (simp_all only: COND13) 
-
-lemma WHILE_False:
-  assumes 1:" \<lceil>\<not>\<^sub>e b\<rceil>" and 2:"is_total (lfp (W b (Rel c)))"  
-  shows "(WHILE b DO c OD) = SKIP"
-  using 1 2  
-  by transfer (auto simp add: WHILE_unfold) 
 
 subsection {*Laws used by tactics*}
 text {*In this section we will design a set of rules that can be used to automatise 
        the process of program optimization.*}
 
-subsubsection {*Assignment rules*}
-text {*We will create a variant rule for @{thm ASN4}. The variant rule in the sequel
-       can be applied naively in an automatic tactic used for optimizing the program.*}
 
-
-lemma ASN4_SE1[symbolic_exec_subst]: 
-  assumes 1: "mwb_lens var" 
-  shows "(var:== exp1 ; var:== \<guillemotleft>exp2\<guillemotright>) = (var:== \<guillemotleft>exp2\<guillemotright>)"
-  using 1 unrest_const[of var exp2] ASN4[of var]
-  by simp
-
-lemma ASN4_SE2[symbolic_exec_subst]: 
-  assumes 1: "mwb_lens var" 
-  shows "(var:== exp1 ; var:== (bop bp (VAR var) \<guillemotleft>exp2\<guillemotright>)) = (var:== (bop bp exp1 \<guillemotleft>exp2\<guillemotright>))"
-  using 1 unrest_const[of var exp2] ASN4_bop1[of var]
-  by auto
-
-lemma ASN4_SE3[symbolic_exec_subst]: 
-  assumes 1: "mwb_lens var" 
-  shows "(var:== exp1 ; var:== (bop bp \<guillemotleft>exp2\<guillemotright> (VAR var))) = (var:== (bop bp \<guillemotleft>exp2\<guillemotright> exp1))"
-  using 1 unrest_const[of var exp2] ASN4_bop2[of var]
-  by auto
-
-lemma ASN4_SE4[symbolic_exec_subst]: 
-  assumes 1: "mwb_lens var"
-  shows "(var:== exp1 ; var:== (trop tp (VAR var) \<guillemotleft>exp2\<guillemotright> \<guillemotleft>exp3\<guillemotright>)) = 
-         (var:== (trop tp exp1 \<guillemotleft>exp2\<guillemotright> \<guillemotleft>exp3\<guillemotright>))"
-  using 1 unrest_const[of var exp2] unrest_const[of var exp3] ASN4_trop1[of var]
-  by auto
-
-lemma ASN4_SE5[symbolic_exec_subst]: 
-  assumes 1: "mwb_lens var"
-  shows "(var:== exp1 ; var:== (trop tp \<guillemotleft>exp2\<guillemotright> (VAR var) \<guillemotleft>exp3\<guillemotright>)) = 
-         (var:== (trop tp \<guillemotleft>exp2\<guillemotright> exp1 \<guillemotleft>exp3\<guillemotright>))"
-  using 1 unrest_const[of var exp2] unrest_const[of var exp3] ASN4_trop2[of var]
-  by auto
-
-lemma ASN4_SE6[symbolic_exec_subst]: 
-  assumes 1: "mwb_lens var"
-  shows "(var:== exp1 ; var:== (trop tp \<guillemotleft>exp2\<guillemotright>  \<guillemotleft>exp3\<guillemotright> (VAR var))) = 
-         (var:== (trop tp \<guillemotleft>exp2\<guillemotright> \<guillemotleft>exp3\<guillemotright> exp1))"
-  using 1 unrest_const[of var exp2] unrest_const[of var exp3] ASN4_trop3[of var]
-  by auto
-
-lemma ASN4_SE7[symbolic_exec_subst]: 
-  assumes 1: "mwb_lens var"
-  shows "(var:== exp1 ; var:== (qtop tp (VAR var) \<guillemotleft>exp2\<guillemotright> \<guillemotleft>exp3\<guillemotright> \<guillemotleft>exp4\<guillemotright>)) = 
-         (var:== (qtop tp exp1 \<guillemotleft>exp2\<guillemotright> \<guillemotleft>exp3\<guillemotright> \<guillemotleft>exp4\<guillemotright>))"
-  using 1 unrest_const[of var exp2] unrest_const[of var exp3] 
-          unrest_const[of var exp4] ASN4_qtop1[of var]
-  by auto
-
-lemma ASN4_SE8[symbolic_exec_subst]: 
-  assumes 1: "mwb_lens var"
-  shows "(var:== exp1 ; var:== (qtop tp \<guillemotleft>exp2\<guillemotright> (VAR var) \<guillemotleft>exp3\<guillemotright> \<guillemotleft>exp4\<guillemotright>)) = 
-         (var:== (qtop tp \<guillemotleft>exp2\<guillemotright> exp1 \<guillemotleft>exp3\<guillemotright> \<guillemotleft>exp4\<guillemotright>))"
-  using 1 unrest_const[of var exp2] unrest_const[of var exp3] 
-          unrest_const[of var exp4] ASN4_qtop2[of var]
-  by auto
-
-lemma ASN4_SE9[symbolic_exec_subst]: 
-  assumes 1: "mwb_lens var"
-  shows "(var:== exp1 ; var:== (qtop tp \<guillemotleft>exp2\<guillemotright>  \<guillemotleft>exp3\<guillemotright> (VAR var) \<guillemotleft>exp4\<guillemotright>)) = 
-         (var:== (qtop tp \<guillemotleft>exp2\<guillemotright> \<guillemotleft>exp3\<guillemotright> exp1 \<guillemotleft>exp4\<guillemotright>))"
-  using 1 unrest_const[of var exp2] unrest_const[of var exp3] 
-          unrest_const[of var exp4] ASN4_qtop3[of var]
-  by auto
-
-lemma ASN4_SE10[symbolic_exec_subst]: 
-  assumes 1: "mwb_lens var"
-  shows "(var:== exp1 ; var:== (qtop tp \<guillemotleft>exp2\<guillemotright> \<guillemotleft>exp3\<guillemotright> \<guillemotleft>exp4\<guillemotright> (VAR var))) = 
-         (var:== (qtop tp \<guillemotleft>exp2\<guillemotright> \<guillemotleft>exp3\<guillemotright> \<guillemotleft>exp4\<guillemotright> exp1))"
-  using 1 unrest_const[of var exp2] unrest_const[of var exp3] 
-          unrest_const[of var exp4] ASN4_qtop4[of var]
-  by auto
-
-lemma ASN11_SE1[symbolic_exec_subst]:
-  assumes 1: "weak_lens var"
-  shows "(IF (bop bp exp \<guillemotleft>exp2\<guillemotright>) THEN (var:== exp ; C1) ELSE (var:== exp ; C2)) =  
-         (var:== exp ; IF (bop bp (VAR var) \<guillemotleft>exp2\<guillemotright>) THEN C1 ELSE C2)"
-  using 1 unfolding subst_upd_var_def
-  by transfer auto
-
-lemma ASN11_SE2[symbolic_exec_subst]:
-  assumes 1: "weak_lens var"
-  shows "(IF (bop bp \<guillemotleft>exp2\<guillemotright> exp1) THEN (var:== exp1 ; C1) ELSE (var:== exp1 ; C2)) = 
-         (var:== exp1 ; IF (bop bp \<guillemotleft>exp2\<guillemotright> (VAR var)) THEN C1 ELSE C2)"
-  using 1 unfolding subst_upd_var_def
-  by transfer auto
-
-lemma ASN11_SE3[symbolic_exec_subst]:
-  assumes 1: "weak_lens var"
-  shows "(IF (trop tp exp1 \<guillemotleft>exp2\<guillemotright> \<guillemotleft>exp3\<guillemotright>) THEN (var:== exp1 ; C1) ELSE (var:== exp1 ; C2))= 
-         (var:== exp1 ; IF (trop tp (VAR var) \<guillemotleft>exp2\<guillemotright> \<guillemotleft>exp3\<guillemotright>) THEN C1 ELSE C2)"
-  using 1 unfolding subst_upd_var_def
-  by transfer auto
-
-lemma ASN11_SE4[symbolic_exec_subst]:
-  assumes 1: "weak_lens var"
-  shows "(IF (trop tp \<guillemotleft>exp2\<guillemotright> exp1 \<guillemotleft>exp3\<guillemotright>) THEN (var:== exp1 ; C1) ELSE (var:== exp1 ; C2))= 
-         (var:== exp1 ; IF (trop tp \<guillemotleft>exp2\<guillemotright> (VAR var) \<guillemotleft>exp3\<guillemotright>) THEN C1 ELSE C2) "
-  using 1 unfolding subst_upd_var_def
-  by transfer auto
-
-lemma ASN11_SE5[symbolic_exec_subst]:
-  assumes 1: "weak_lens var"
-  shows "(IF (trop bp \<guillemotleft>exp2\<guillemotright> \<guillemotleft>exp3\<guillemotright> exp1) THEN (var:== exp1 ; C1) ELSE (var:== exp1 ; C2)) = 
-         (var:== exp1 ; IF (trop bp \<guillemotleft>exp2\<guillemotright> \<guillemotleft>exp3\<guillemotright> (VAR var)) THEN C1 ELSE C2)"
-  using 1 unfolding subst_upd_var_def
-  by transfer auto
-
-lemma ASN11_SE6[symbolic_exec_subst]:
-  assumes 1: "weak_lens var" 
-  shows "(IF (qtop tp exp1 \<guillemotleft>exp2\<guillemotright> \<guillemotleft>exp3\<guillemotright> \<guillemotleft>exp4\<guillemotright>) THEN (var:== exp1 ; C1) ELSE (var:== exp1 ; C2)) =
-         (var:== exp1 ; IF (qtop tp (VAR var) \<guillemotleft>exp2\<guillemotright> \<guillemotleft>exp3\<guillemotright> \<guillemotleft>exp4\<guillemotright>) THEN C1 ELSE C2)"
-  using 1 unfolding subst_upd_var_def
-  by transfer auto
-
-lemma ASN11_SE7[symbolic_exec_subst]:
-  assumes 1: "weak_lens var"
-  shows "(IF (qtop tp \<guillemotleft>exp2\<guillemotright> exp1 \<guillemotleft>exp3\<guillemotright> \<guillemotleft>exp4\<guillemotright>) THEN (var:== exp1 ; C1) ELSE (var:== exp1 ; C2)) = 
-         (var:== exp1 ; IF (qtop tp \<guillemotleft>exp2\<guillemotright> (VAR var) \<guillemotleft>exp3\<guillemotright> \<guillemotleft>exp4\<guillemotright>) THEN C1 ELSE C2)"
-  using 1 unfolding subst_upd_var_def
-  by transfer auto
-
-lemma ASN11_SE8[symbolic_exec_subst]:
-  assumes 1: "weak_lens var" 
-  shows "(IF (qtop bp \<guillemotleft>exp2\<guillemotright> \<guillemotleft>exp3\<guillemotright> exp1 \<guillemotleft>exp4\<guillemotright>) THEN (var:== exp1 ; C1) ELSE (var:== exp1 ; C2)) =  
-         (var:== exp1 ; IF (qtop bp \<guillemotleft>exp2\<guillemotright> \<guillemotleft>exp3\<guillemotright> (VAR var) \<guillemotleft>exp4\<guillemotright>) THEN C1 ELSE C2)"
-  using 1 unfolding subst_upd_var_def
-  by transfer auto
-
-lemma ASN11_SE9[symbolic_exec_subst]:
-  assumes 1: "weak_lens var" and 2: "var \<sharp> exp2" and 3: "var \<sharp> exp3" and 4: "var \<sharp> exp4"
-  shows "(IF (qtop bp \<guillemotleft>exp2\<guillemotright> \<guillemotleft>exp3\<guillemotright> \<guillemotleft>exp4\<guillemotright> exp1) THEN (var:== exp1 ; C1) ELSE (var:== exp1 ; C2)) = 
-         (var:== exp1 ; IF (qtop bp \<guillemotleft>exp2\<guillemotright> \<guillemotleft>exp3\<guillemotright> \<guillemotleft>exp4\<guillemotright> (VAR var)) THEN C1 ELSE C2)"
-  using 1 unfolding subst_upd_var_def
-  by transfer auto
-
-lemma ASN13_SE1[symbolic_exec_subst]:
-  assumes 1: "mwb_lens var"
-  shows "((var:== E); 
-          IF bop F (VAR var) \<guillemotleft>exp\<guillemotright> THEN (var:== (bop F (VAR var) \<guillemotleft>exp\<guillemotright>)) ELSE (var:== (bop G (VAR var) \<guillemotleft>exp\<guillemotright>))) =
-         (var:== (trop If (bop F E \<guillemotleft>exp\<guillemotright>) (bop F E \<guillemotleft>exp\<guillemotright>) (bop G E \<guillemotleft>exp\<guillemotright>)))" 
-  using 1 unfolding subst_upd_var_def
-  by transfer auto
-
-lemma ASN13_SE2[symbolic_exec_subst]:
-  assumes 1: "mwb_lens var"
-  shows "((var:== E); 
-          IF bop F \<guillemotleft>exp\<guillemotright> (VAR var)  THEN (var:== (bop F \<guillemotleft>exp\<guillemotright> (VAR var))) ELSE (var:== (bop G \<guillemotleft>exp\<guillemotright> (VAR var)))) =
-         (var:== (trop If (bop F \<guillemotleft>exp\<guillemotright> E) (bop F \<guillemotleft>exp\<guillemotright> E) (bop G \<guillemotleft>exp\<guillemotright> E)))" 
-  using 1 unrest_const[of var exp] ASN13_bop[of var] 
-  by auto
-
-lemma ASN13_SE3[symbolic_exec_subst]:
-  assumes 1: "mwb_lens var"
-  shows "((var:== E); 
-          IF bop F (VAR var) \<guillemotleft>exp1\<guillemotright> THEN (var:== (bop F (VAR var) \<guillemotleft>exp1\<guillemotright>)) ELSE (var:== (bop G (VAR var) \<guillemotleft>exp2\<guillemotright>))) =
-         (var:== (trop If (bop F E \<guillemotleft>exp1\<guillemotright>) (bop F E \<guillemotleft>exp1\<guillemotright>) (bop G E \<guillemotleft>exp2\<guillemotright>)))" 
-  using 1 unrest_const[of var exp1] unrest_const[of var exp2] ASN13_bop2[of var] 
-  by auto
-
-lemma ASN13_SE4[symbolic_exec_subst]:
-  assumes 1: "mwb_lens var"
-  shows "((var:== E); 
-          IF bop F (VAR var) \<guillemotleft>exp1\<guillemotright> THEN (var:== (bop F (VAR var) \<guillemotleft>exp1\<guillemotright>)) ELSE (var:== (bop G \<guillemotleft>exp2\<guillemotright> (VAR var)))) =
-         (var:== (trop If (bop F E \<guillemotleft>exp1\<guillemotright>) (bop F E \<guillemotleft>exp1\<guillemotright>) (bop G \<guillemotleft>exp2\<guillemotright> E)))" 
-  using 1 unrest_const[of var exp1] unrest_const[of var exp2] ASN13_bop4[of var] 
-  by auto
-
-lemma ASN13_SE5[symbolic_exec_subst]:
-  assumes 1: "mwb_lens var"
-  shows "((var:== E); 
-          IF bop F \<guillemotleft>exp1\<guillemotright> (VAR var) THEN (var:== (bop F \<guillemotleft>exp1\<guillemotright> (VAR var))) ELSE (var:== (bop G (VAR var) \<guillemotleft>exp2\<guillemotright>))) =
-         (var:== (trop If (bop F \<guillemotleft>exp1\<guillemotright> E) (bop F \<guillemotleft>exp1\<guillemotright> E) (bop G E \<guillemotleft>exp2\<guillemotright>)))" 
-  using 1 unrest_const[of var exp1] unrest_const[of var exp2] ASN13_bop5[of var] 
-  by auto
-
-lemma ASN13_SE6[symbolic_exec_subst]:
-  assumes 1: "mwb_lens var"
-  shows "((var:== E); 
-          IF bop F \<guillemotleft>exp1\<guillemotright> (VAR var) THEN (var:== (bop F \<guillemotleft>exp1\<guillemotright> (VAR var))) ELSE (var:== (bop G \<guillemotleft>exp2\<guillemotright> (VAR var)))) =
-         (var:== (trop If (bop F \<guillemotleft>exp1\<guillemotright> E) (bop F \<guillemotleft>exp1\<guillemotright> E) (bop G \<guillemotleft>exp2\<guillemotright> E)))" 
-  using 1 unrest_const[of var exp1] unrest_const[of var exp2] ASN13_bop6[of var] 
-  by auto                                                           
-
-lemma ASN13_SE7[symbolic_exec_subst]:
-  assumes 1: "mwb_lens var"
-  shows "((var:== E); 
-          IF trop F \<guillemotleft>exp1\<guillemotright> \<guillemotleft>exp2\<guillemotright> (VAR var)  THEN (var:== (trop F \<guillemotleft>exp1\<guillemotright> \<guillemotleft>exp2\<guillemotright> (VAR var))) ELSE (var:== (trop G \<guillemotleft>exp1\<guillemotright> \<guillemotleft>exp2\<guillemotright> (VAR var)))) =
-         (var:== (trop If (trop F \<guillemotleft>exp1\<guillemotright> \<guillemotleft>exp2\<guillemotright> E) (trop F \<guillemotleft>exp1\<guillemotright> \<guillemotleft>exp2\<guillemotright> E) (trop G \<guillemotleft>exp1\<guillemotright> \<guillemotleft>exp2\<guillemotright> E)))" 
-  using 1 unrest_const[of var exp1] unrest_const[of var exp2] ASN13_trop[of var] 
-  by auto                                                           
-
-lemma ASN13_SE8[symbolic_exec_subst]:
-  assumes 1: "mwb_lens var"
-  shows "((var:== E); 
-          IF trop F \<guillemotleft>exp1\<guillemotright> (VAR var) \<guillemotleft>exp2\<guillemotright> THEN (var:== (trop F \<guillemotleft>exp1\<guillemotright> (VAR var) \<guillemotleft>exp2\<guillemotright>)) ELSE (var:== (trop G \<guillemotleft>exp1\<guillemotright> (VAR var) \<guillemotleft>exp2\<guillemotright>))) =
-         (var:== (trop If (trop F \<guillemotleft>exp1\<guillemotright> E \<guillemotleft>exp2\<guillemotright>) (trop F \<guillemotleft>exp1\<guillemotright> E \<guillemotleft>exp2\<guillemotright>) (trop G \<guillemotleft>exp1\<guillemotright> E \<guillemotleft>exp2\<guillemotright>)))" 
-  using 1 unrest_const[of var exp1] unrest_const[of var exp2] ASN13_trop1[of var] 
-  by auto
-
-lemma ASN13_SE9[symbolic_exec_subst]:
-  assumes 1: "mwb_lens var"
-  shows "((var:== E); 
-          IF trop F (VAR var) \<guillemotleft>exp1\<guillemotright> \<guillemotleft>exp2\<guillemotright> THEN (var:== (trop F (VAR var) \<guillemotleft>exp1\<guillemotright> \<guillemotleft>exp2\<guillemotright>)) ELSE (var:== (trop G (VAR var) \<guillemotleft>exp1\<guillemotright> \<guillemotleft>exp2\<guillemotright>))) =
-         (var:== (trop If (trop F E \<guillemotleft>exp1\<guillemotright> \<guillemotleft>exp2\<guillemotright>) (trop F E \<guillemotleft>exp1\<guillemotright> \<guillemotleft>exp2\<guillemotright>) (trop G E \<guillemotleft>exp1\<guillemotright> \<guillemotleft>exp2\<guillemotright>)))" 
-  using 1 unrest_const[of var exp1] unrest_const[of var exp2] ASN13_trop2[of var] 
-  by auto 
-
-lemma ASN13_SE10[symbolic_exec_subst]:
-  assumes 1: "mwb_lens var" 
-  shows "((var:== E); 
-          IF trop F \<guillemotleft>exp1\<guillemotright> \<guillemotleft>exp2\<guillemotright> (VAR var) THEN (var:== (trop F \<guillemotleft>exp1\<guillemotright> \<guillemotleft>exp2\<guillemotright> (VAR var))) ELSE (var:== (trop G \<guillemotleft>exp3\<guillemotright> \<guillemotleft>exp4\<guillemotright> (VAR var)))) =
-         (var:== (trop If (trop F \<guillemotleft>exp1\<guillemotright> \<guillemotleft>exp2\<guillemotright> E) (trop F \<guillemotleft>exp1\<guillemotright> \<guillemotleft>exp2\<guillemotright> E) (trop G \<guillemotleft>exp3\<guillemotright> \<guillemotleft>exp4\<guillemotright> E)))" 
-  using 1 unrest_const[of var exp1] unrest_const[of var exp2] ASN13_trop3[of var]
-          unrest_const[of var exp3] unrest_const[of var exp4] 
-  by auto
-
-lemma ASN13_SE11[symbolic_exec_subst]:
-  assumes 1: "mwb_lens var" 
-  shows "((var:== E); 
-          IF trop F \<guillemotleft>exp1\<guillemotright> (VAR var) \<guillemotleft>exp2\<guillemotright> THEN (var:== (trop F \<guillemotleft>exp1\<guillemotright> (VAR var) \<guillemotleft>exp2\<guillemotright>)) ELSE (var:== (trop G \<guillemotleft>exp3\<guillemotright> (VAR var) \<guillemotleft>exp4\<guillemotright>))) =
-         (var:== (trop If (trop F \<guillemotleft>exp1\<guillemotright> E \<guillemotleft>exp2\<guillemotright>) (trop F \<guillemotleft>exp1\<guillemotright> E \<guillemotleft>exp2\<guillemotright>) (trop G \<guillemotleft>exp3\<guillemotright> E \<guillemotleft>exp4\<guillemotright>)))" 
-  using 1 unrest_const[of var exp1] unrest_const[of var exp2] ASN13_trop4[of var]
-          unrest_const[of var exp3] unrest_const[of var exp4] 
-  by auto
-
-lemma ASN13_SE12[symbolic_exec_subst]:
-  assumes 1: "mwb_lens var"
-  shows "((var:== E); 
-          IF trop F (VAR var) \<guillemotleft>exp1\<guillemotright> \<guillemotleft>exp2\<guillemotright> THEN (var:== (trop F (VAR var) \<guillemotleft>exp1\<guillemotright> \<guillemotleft>exp2\<guillemotright>)) ELSE (var:== (trop G (VAR var) \<guillemotleft>exp3\<guillemotright> \<guillemotleft>exp4\<guillemotright>))) =
-         (var:== (trop If (trop F E \<guillemotleft>exp1\<guillemotright> \<guillemotleft>exp2\<guillemotright>) (trop F E \<guillemotleft>exp1\<guillemotright> \<guillemotleft>exp2\<guillemotright>) (trop G E \<guillemotleft>exp3\<guillemotright> \<guillemotleft>exp4\<guillemotright>)))" 
-  using 1 unrest_const[of var exp1] unrest_const[of var exp2] ASN13_trop5[of var]
-          unrest_const[of var exp3] unrest_const[of var exp4] 
-  by auto
 
 end
