WP1-Programming-Languages-Semantics/WP11-C-semantics/src/IMP-Lenses/utp/utp_urel_setup.thy
@@ -1,0 +1,83 @@
+section {* UTP variables *}
+
+theory utp_urel_setup
+  imports utp_lift
+begin
+ named_theorems urel_defs
+
+text {*
+  We set up several automatic tactics that recast theorems on UTP predicates
+  into equivalent HOL predicates, eliminating artefacts of the mechanisation
+  as much as this is possible. Our approach is first to unfold all relevant
+  definition of the UTP predicate model, then perform a transfer, and finally
+  simplify by using lens and variable definitions, the split laws of alphabet
+  records, and interpretation laws to convert record-based state spaces into
+  products. The definition of the methods is facilitated by the Eisbach tool.
+*}
+
+text {* Without re-interpretation of lens types in state spaces (legacy). *}
+
+method rel_simp' = (
+  (unfold upred_defs urel_defs)?,
+  (transfer),
+  (simp add: fun_eq_iff relcomp_unfold OO_def
+    lens_defs upred_defs (*alpha_splits*) Product_Type.split_beta)?,
+  (clarsimp)?)
+
+text {* Variations that adjoin @{method rel_simp'} with automatic tactics. *}
+
+method rel_auto' = (rel_simp', auto?)
+method rel_blast' = (rel_simp'; blast)
+
+text {* With reinterpretation of lens types in state spaces (default). *}
+
+method rel_simp = (
+  (unfold upred_defs urel_defs)?,
+  (transfer),
+  (simp add: fun_eq_iff relcomp_unfold OO_def
+    lens_defs upred_defs (*alpha_splits*) Product_Type.split_beta)?,
+  (simp add: lens_interp_laws)?,
+  (clarsimp)?)
+
+text {* Variations that adjoin @{method rel_simp} with automatic tactics. *}
+
+method rel_auto = (rel_simp, auto?)
+method rel_blast = (rel_simp; blast)
+
+
+definition in\<alpha> :: "('\<alpha>, '\<alpha> \<times> '\<beta>) uvar" where
+"in\<alpha> = \<lparr> lens_get = fst, lens_put = \<lambda> (A, A') v. (v, A') \<rparr>"
+
+definition out\<alpha> :: "('\<beta>, '\<alpha> \<times> '\<beta>) uvar" where
+"out\<alpha> = \<lparr> lens_get = snd, lens_put = \<lambda> (A, A') v. (A, v) \<rparr>"
+
+declare in\<alpha>_def [urel_defs]
+declare out\<alpha>_def [urel_defs]
+
+lemma var_in_alpha [simp]: "x ;\<^sub>L in\<alpha> = ivar x"
+  by (simp add: fst_lens_def in\<alpha>_def in_var_def)
+
+lemma var_out_alpha [simp]: "x ;\<^sub>L out\<alpha> = ovar x"
+  by (simp add: out\<alpha>_def out_var_def snd_lens_def)
+
+lemma out_alpha_in_indep [simp]:
+  "out\<alpha> \<bowtie> in_var x" "in_var x \<bowtie> out\<alpha>"
+  by (simp_all add: in_var_def out\<alpha>_def lens_indep_def fst_lens_def lens_comp_def)
+
+lemma in_alpha_out_indep [simp]:
+  "in\<alpha> \<bowtie> out_var x" "out_var x \<bowtie> in\<alpha>"
+  by (simp_all add: in_var_def in\<alpha>_def lens_indep_def fst_lens_def lens_comp_def)
+
+text {* The alphabet of a relation consists of the input and output portions *}
+
+lemma alpha_in_out:
+  "\<Sigma> \<approx>\<^sub>L in\<alpha> +\<^sub>L out\<alpha>"
+  by (metis fst_lens_def fst_snd_id_lens in\<alpha>_def lens_equiv_refl out\<alpha>_def snd_lens_def)
+
+abbreviation usubst_rel_lift :: "'\<alpha> usubst \<Rightarrow> ('\<alpha> \<times> '\<beta>) usubst" ("\<lceil>_\<rceil>\<^sub>s") where
+"\<lceil>\<sigma>\<rceil>\<^sub>s \<equiv> \<sigma> \<oplus>\<^sub>s in\<alpha>"
+
+abbreviation usubst_rel_drop :: "('\<alpha> \<times> '\<alpha>) usubst \<Rightarrow> '\<alpha> usubst" ("\<lfloor>_\<rfloor>\<^sub>s") where
+"\<lfloor>\<sigma>\<rfloor>\<^sub>s \<equiv> \<sigma> \<restriction>\<^sub>s in\<alpha>"
+
+end
